<?xml version="1.0"?>


<!DOCTYPE rdf:RDF [
    <!ENTITY owl "http://www.w3.org/2002/07/owl#" >
    <!ENTITY dc "http://purl.org/dc/elements/1.1/" >
    <!ENTITY xsd "http://www.w3.org/2001/XMLSchema#" >
    <!ENTITY error "http://org.semanticweb.owlapi/error#" >
    <!ENTITY rdfs "http://www.w3.org/2000/01/rdf-schema#" >
    <!ENTITY ns4 "http://library.ucsd.edu/ontology/dams/" >
    <!ENTITY rdf "http://www.w3.org/1999/02/22-rdf-syntax-ns#" >
]>


<rdf:RDF xmlns="&ns4;#"
     xml:base="http://library.ucsd.edu/ontology/dams/"
     xmlns:dc="http://purl.org/dc/elements/1.1/"
     xmlns:rdfs="http://www.w3.org/2000/01/rdf-schema#"
     xmlns:ns4="http://library.ucsd.edu/ontology/dams/"
     xmlns:error="http://org.semanticweb.owlapi/error#"
     xmlns:owl="http://www.w3.org/2002/07/owl#"
     xmlns:xsd="http://www.w3.org/2001/XMLSchema#"
     xmlns:rdf="http://www.w3.org/1999/02/22-rdf-syntax-ns#">
    <owl:Ontology rdf:about="http://library.ucsd.edu/ontology/dams/">
        <rdfs:label>DAMS Data Model</rdfs:label>
        <rdfs:comment>OWL ontology for DAMS content.  Developed at The UC San Diego
      Library by Esm√© Cowles, Matt Critchlow, Arwen Hutt, Longshou Situ and Brad
      Westbrook.</rdfs:comment>
    </owl:Ontology>
    


    <!-- 
    ///////////////////////////////////////////////////////////////////////////////////////
    //
    // Annotation properties
    //
    ///////////////////////////////////////////////////////////////////////////////////////
     -->

    


    <!-- 
    ///////////////////////////////////////////////////////////////////////////////////////
    //
    // Datatypes
    //
    ///////////////////////////////////////////////////////////////////////////////////////
     -->

    


    <!-- http://www.w3.org/2001/XMLSchema#date -->

    <rdfs:Datatype rdf:about="&xsd;date"/>
    


    <!-- 
    ///////////////////////////////////////////////////////////////////////////////////////
    //
    // Object Properties
    //
    ///////////////////////////////////////////////////////////////////////////////////////
     -->

    


    <!-- http://library.ucsd.edu/ontology/dams/#cartographics -->

    <owl:ObjectProperty rdf:about="&ns4;#cartographics">
        <rdfs:comment>Links a Subject to a Cartographics.</rdfs:comment>
        <rdfs:range rdf:resource="&ns4;#Cartographics"/>
        <rdfs:domain rdf:resource="&ns4;#Subject"/>
    </owl:ObjectProperty>
    


    <!-- http://library.ucsd.edu/ontology/dams/#collection -->

    <owl:ObjectProperty rdf:about="&ns4;#collection">
        <rdfs:comment>Links from a child Collection to its parent Collection.</rdfs:comment>
        <rdfs:range rdf:resource="&ns4;#Collection"/>
        <owl:inverseOf rdf:resource="&ns4;#hasCollection"/>
        <rdfs:domain>
            <owl:Class>
                <owl:unionOf rdf:parseType="Collection">
                    <rdf:Description rdf:about="&ns4;#Collection"/>
                    <rdf:Description rdf:about="&ns4;#Object"/>
                </owl:unionOf>
            </owl:Class>
        </rdfs:domain>
    </owl:ObjectProperty>
    


    <!-- http://library.ucsd.edu/ontology/dams/#component -->

    <owl:ObjectProperty rdf:about="&ns4;#component">
        <rdfs:label>component</rdfs:label>
        <rdfs:comment>Links a Component or File to the Component that contains it.</rdfs:comment>
        <rdfs:range rdf:resource="&ns4;#Component"/>
        <rdfs:domain>
            <owl:Class>
                <owl:unionOf rdf:parseType="Collection">
                    <rdf:Description rdf:about="&ns4;#Component"/>
                    <rdf:Description rdf:about="&ns4;#File"/>
                </owl:unionOf>
            </owl:Class>
        </rdfs:domain>
    </owl:ObjectProperty>
    


    <!-- http://library.ucsd.edu/ontology/dams/#copyright -->

    <owl:ObjectProperty rdf:about="&ns4;#copyright">
        <rdfs:comment>Links an item to a Copyright statement.</rdfs:comment>
        <rdfs:range rdf:resource="&ns4;#Copyright"/>
        <rdfs:domain>
            <owl:Class>
                <owl:unionOf rdf:parseType="Collection">
                    <rdf:Description rdf:about="&ns4;#Component"/>
                    <rdf:Description rdf:about="&ns4;#Object"/>
                </owl:unionOf>
            </owl:Class>
        </rdfs:domain>
    </owl:ObjectProperty>
    


    <!-- http://library.ucsd.edu/ontology/dams/#date -->

    <owl:ObjectProperty rdf:about="&ns4;#date">
        <rdfs:label>date</rdfs:label>
        <rdfs:comment>Links an item to a Date.</rdfs:comment>
        <rdfs:range rdf:resource="&ns4;#Date"/>
        <rdfs:domain>
            <owl:Class>
                <owl:unionOf rdf:parseType="Collection">
                    <rdf:Description rdf:about="&ns4;#Copyright"/>
                    <rdf:Description rdf:about="&ns4;#DAMSResource"/>
                </owl:unionOf>
            </owl:Class>
        </rdfs:domain>
    </owl:ObjectProperty>
    


    <!-- http://library.ucsd.edu/ontology/dams/#event -->

    <owl:ObjectProperty rdf:about="&ns4;#event">
        <rdfs:label>event</rdfs:label>
        <rdfs:comment>Links a metadata record to an Event that is related to it.</rdfs:comment>
        <rdfs:range rdf:resource="&ns4;#DAMSEvent"/>
        <rdfs:domain rdf:resource="&ns4;#DAMSThing"/>
    </owl:ObjectProperty>
    


    <!-- http://library.ucsd.edu/ontology/dams/#hasCollection -->

    <owl:ObjectProperty rdf:about="&ns4;#hasCollection">
        <rdfs:comment>Links from a parent Collection to a child Collection.</rdfs:comment>
        <rdfs:range rdf:resource="&ns4;#Collection"/>
        <rdfs:domain rdf:resource="&ns4;#Collection"/>
    </owl:ObjectProperty>
    


    <!-- http://library.ucsd.edu/ontology/dams/#hasComponent -->

    <owl:ObjectProperty rdf:about="&ns4;#hasComponent">
        <rdfs:label>hasComponent</rdfs:label>
        <rdfs:comment>Links from a parent Component or Object to a Component it contains.</rdfs:comment>
        <rdfs:range rdf:resource="&ns4;#Component"/>
        <owl:inverseOf rdf:resource="&ns4;#component"/>
        <rdfs:domain>
            <owl:Class>
                <owl:unionOf rdf:parseType="Collection">
                    <rdf:Description rdf:about="&ns4;#Component"/>
                    <rdf:Description rdf:about="&ns4;#Object"/>
                </owl:unionOf>
            </owl:Class>
        </rdfs:domain>
    </owl:ObjectProperty>
    


    <!-- http://library.ucsd.edu/ontology/dams/#hasFile -->

    <owl:ObjectProperty rdf:about="&ns4;#hasFile">
        <rdfs:label>hasFile</rdfs:label>
        <rdfs:comment>Links from a parent Component or Object to a File it contains.</rdfs:comment>
        <rdfs:range rdf:resource="&ns4;#File"/>
        <rdfs:domain>
            <owl:Class>
                <owl:unionOf rdf:parseType="Collection">
                    <rdf:Description rdf:about="&ns4;#Component"/>
                    <rdf:Description rdf:about="&ns4;#Object"/>
                </owl:unionOf>
            </owl:Class>
        </rdfs:domain>
    </owl:ObjectProperty>
    


    <!-- http://library.ucsd.edu/ontology/dams/#hasObject -->

    <owl:ObjectProperty rdf:about="&ns4;#hasObject">
        <rdfs:label>hasObject</rdfs:label>
        <rdfs:comment>Links from a parent Collection or Repository to an Object it contains.</rdfs:comment>
        <rdfs:range rdf:resource="&ns4;#Object"/>
        <rdfs:domain>
            <owl:Class>
                <owl:unionOf rdf:parseType="Collection">
                    <rdf:Description rdf:about="&ns4;#Collection"/>
                    <rdf:Description rdf:about="&ns4;#Repository"/>
                </owl:unionOf>
            </owl:Class>
        </rdfs:domain>
    </owl:ObjectProperty>
    


    <!-- http://library.ucsd.edu/ontology/dams/#hasPart -->

    <owl:ObjectProperty rdf:about="&ns4;#hasPart">
        <rdfs:comment>Links from a parent ProvenanceCollection to a child ProvenanceCollectionPart.</rdfs:comment>
        <rdfs:domain rdf:resource="&ns4;ProvenanceCollection"/>
        <rdfs:range rdf:resource="&ns4;ProvenanceCollectionPart"/>
    </owl:ObjectProperty>
    


    <!-- http://library.ucsd.edu/ontology/dams/#hasProvenanceCollection -->

    <owl:ObjectProperty rdf:about="&ns4;#hasProvenanceCollection">
        <rdfs:comment>Links from a parent Collection to a child ProvenanceCollection</rdfs:comment>
        <rdfs:range rdf:resource="&ns4;ProvenanceCollection"/>
        <rdfs:domain rdf:resource="&ns4;#Collection"/>
    </owl:ObjectProperty>
    


    <!-- http://library.ucsd.edu/ontology/dams/#language -->

    <owl:ObjectProperty rdf:about="&ns4;#language">
        <rdfs:label>language</rdfs:label>
        <rdfs:comment>Links an item to a Language.</rdfs:comment>
        <rdfs:range rdf:resource="&ns4;#Language"/>
        <rdfs:domain>
            <owl:Class>
                <owl:unionOf rdf:parseType="Collection">
                    <rdf:Description rdf:about="&ns4;#DAMSResource"/>
                    <rdf:Description rdf:about="&ns4;#Title"/>
                </owl:unionOf>
            </owl:Class>
        </rdfs:domain>
    </owl:ObjectProperty>
    


    <!-- http://library.ucsd.edu/ontology/dams/#license -->

    <owl:ObjectProperty rdf:about="&ns4;#license">
        <rdfs:comment>Links an item to a License.</rdfs:comment>
        <rdfs:range rdf:resource="&ns4;#License"/>
        <rdfs:domain>
            <owl:Class>
                <owl:unionOf rdf:parseType="Collection">
                    <rdf:Description rdf:about="&ns4;#Component"/>
                    <rdf:Description rdf:about="&ns4;#Object"/>
                </owl:unionOf>
            </owl:Class>
        </rdfs:domain>
    </owl:ObjectProperty>
    


    <!-- http://library.ucsd.edu/ontology/dams/#name -->

    <owl:ObjectProperty rdf:about="&ns4;#name">
        <rdfs:label>name</rdfs:label>
        <rdfs:comment>Links a Relationship to a Name.</rdfs:comment>
        <rdfs:range rdf:resource="&ns4;#Name"/>
        <rdfs:domain>
            <owl:Class>
                <owl:unionOf rdf:parseType="Collection">
                    <rdf:Description rdf:about="&ns4;#Relationship"/>
                    <rdf:Description rdf:about="&ns4;#Subject"/>
                </owl:unionOf>
            </owl:Class>
        </rdfs:domain>
    </owl:ObjectProperty>
    


    <!-- http://library.ucsd.edu/ontology/dams/#note -->

    <owl:ObjectProperty rdf:about="&ns4;#note">
        <rdfs:label>note</rdfs:label>
        <rdfs:comment>Links an item to a Note.</rdfs:comment>
        <rdfs:domain rdf:resource="&ns4;#DAMSResource"/>
        <rdfs:range rdf:resource="&ns4;#Note"/>
    </owl:ObjectProperty>
    


    <!-- http://library.ucsd.edu/ontology/dams/#object -->

    <owl:ObjectProperty rdf:about="&ns4;#object">
        <rdfs:label>object</rdfs:label>
        <rdfs:comment>Links a Component or File to the Object that contains it.</rdfs:comment>
        <rdfs:range rdf:resource="&ns4;#Object"/>
        <rdfs:domain>
            <owl:Class>
                <owl:unionOf rdf:parseType="Collection">
                    <rdf:Description rdf:about="&ns4;#Component"/>
                    <rdf:Description rdf:about="&ns4;#File"/>
                </owl:unionOf>
            </owl:Class>
        </rdfs:domain>
    </owl:ObjectProperty>
    


    <!-- http://library.ucsd.edu/ontology/dams/#otherRights -->

    <owl:ObjectProperty rdf:about="&ns4;#otherRights">
        <rdfs:comment>Links an item to an OtherRights.</rdfs:comment>
        <rdfs:range rdf:resource="&ns4;#OtherRights"/>
        <rdfs:domain>
            <owl:Class>
                <owl:unionOf rdf:parseType="Collection">
                    <rdf:Description rdf:about="&ns4;#Component"/>
                    <rdf:Description rdf:about="&ns4;#File"/>
                    <rdf:Description rdf:about="&ns4;#Object"/>
                </owl:unionOf>
            </owl:Class>
        </rdfs:domain>
    </owl:ObjectProperty>
    


    <!-- http://library.ucsd.edu/ontology/dams/#provenanceCollection -->

    <owl:ObjectProperty rdf:about="&ns4;#provenanceCollection">
        <rdfs:comment>Links from a child ProvenanceCollectionPart to a parent ProvenanceCollection.</rdfs:comment>
        <rdfs:range rdf:resource="&ns4;ProvenanceCollection"/>
        <rdfs:domain rdf:resource="&ns4;ProvenanceCollectionPart"/>
    </owl:ObjectProperty>
    


    <!-- http://library.ucsd.edu/ontology/dams/#relatedCollection -->

    <owl:ObjectProperty rdf:about="&ns4;#relatedCollection">
        <rdfs:label>relatedCollection</rdfs:label>
        <rdfs:comment>Peer collection relationship.</rdfs:comment>
        <rdfs:domain rdf:resource="&ns4;#Collection"/>
        <rdfs:range rdf:resource="&ns4;#Collection"/>
    </owl:ObjectProperty>
    


    <!-- http://library.ucsd.edu/ontology/dams/#relatedResource -->

    <owl:ObjectProperty rdf:about="&ns4;#relatedResource">
        <rdfs:label>relatedResource</rdfs:label>
        <rdfs:comment>Links an item to a RelatedResource.</rdfs:comment>
        <rdfs:domain rdf:resource="&ns4;#DAMSResource"/>
        <rdfs:range rdf:resource="&ns4;#RelatedResource"/>
    </owl:ObjectProperty>
    


    <!-- http://library.ucsd.edu/ontology/dams/#relatedTitle -->

    <owl:ObjectProperty rdf:about="&ns4;#relatedTitle">
        <rdfs:label>relatedTitle</rdfs:label>
        <rdfs:comment>Links a Title to another form of the same Title (e.g., transliterated,
       translated, abbreviated, etc.).</rdfs:comment>
        <rdfs:range rdf:resource="&ns4;#Title"/>
        <rdfs:domain rdf:resource="&ns4;#Title"/>
    </owl:ObjectProperty>
    


    <!-- http://library.ucsd.edu/ontology/dams/#relationship -->

    <owl:ObjectProperty rdf:about="&ns4;#relationship">
        <rdfs:label>relationship</rdfs:label>
        <rdfs:comment>Links an item to a Relationship.</rdfs:comment>
        <rdfs:range rdf:resource="&ns4;#Relationship"/>
        <rdfs:domain>
            <owl:Class>
                <owl:unionOf rdf:parseType="Collection">
                    <rdf:Description rdf:about="&ns4;#Copyright"/>
                    <rdf:Description rdf:about="&ns4;#DAMSResource"/>
                    <rdf:Description rdf:about="&ns4;#License"/>
                    <rdf:Description rdf:about="&ns4;#OtherRights"/>
                </owl:unionOf>
            </owl:Class>
        </rdfs:domain>
    </owl:ObjectProperty>
    


    <!-- http://library.ucsd.edu/ontology/dams/#repository -->

    <owl:ObjectProperty rdf:about="&ns4;#repository">
        <rdf:type rdf:resource="&owl;FunctionalProperty"/>
        <rdfs:comment>Links an Object to the Repository that manages it.</rdfs:comment>
        <rdfs:domain rdf:resource="&ns4;#Object"/>
        <rdfs:range rdf:resource="&ns4;#Repository"/>
    </owl:ObjectProperty>
    


    <!-- http://library.ucsd.edu/ontology/dams/#rightsAction -->

    <owl:ObjectProperty rdf:about="&ns4;#rightsAction">
        <rdfs:comment>Links a Rights element to an actionable RightsAction.</rdfs:comment>
        <rdfs:domain rdf:resource="&ns4;#Rights"/>
        <rdfs:range rdf:resource="&ns4;#RightsAction"/>
    </owl:ObjectProperty>
    


    <!-- http://library.ucsd.edu/ontology/dams/#role -->

    <owl:ObjectProperty rdf:about="&ns4;#role">
        <rdfs:comment>Links a Relationship to a Role.</rdfs:comment>
        <rdfs:domain rdf:resource="&ns4;#Relationship"/>
        <rdfs:range rdf:resource="&ns4;#Role"/>
    </owl:ObjectProperty>
    


    <!-- http://library.ucsd.edu/ontology/dams/#scopeContentNote -->

    <owl:ObjectProperty rdf:about="&ns4;#scopeContentNote">
        <rdfs:label>scopeContentNote</rdfs:label>
        <rdfs:comment>This should be a literal, not a class.</rdfs:comment>
        <rdfs:comment>Links a Collection to a ScopeContentNote.</rdfs:comment>
        <rdfs:domain rdf:resource="&ns4;#Collection"/>
        <rdfs:range rdf:resource="&ns4;#ScopeContentNote"/>
        <rdfs:subPropertyOf rdf:resource="&ns4;#note"/>
    </owl:ObjectProperty>
    


    <!-- http://library.ucsd.edu/ontology/dams/#sourceCapture -->

    <owl:ObjectProperty rdf:about="&ns4;#sourceCapture">
        <rdfs:label>sourceCapture</rdfs:label>
        <rdfs:comment>Links a File to SourceCapture describing its digitization.</rdfs:comment>
        <rdfs:domain rdf:resource="&ns4;#File"/>
        <rdfs:range rdf:resource="&ns4;#SourceCapture"/>
    </owl:ObjectProperty>
    


    <!-- http://library.ucsd.edu/ontology/dams/#statute -->

    <owl:ObjectProperty rdf:about="&ns4;#statute">
        <rdfs:label>statute</rdfs:label>
        <rdfs:comment>Links an item to a Statute.</rdfs:comment>
        <rdfs:range rdf:resource="&ns4;#Statute"/>
        <rdfs:domain>
            <owl:Class>
                <owl:unionOf rdf:parseType="Collection">
                    <rdf:Description rdf:about="&ns4;#Component"/>
                    <rdf:Description rdf:about="&ns4;#Object"/>
                </owl:unionOf>
            </owl:Class>
        </rdfs:domain>
    </owl:ObjectProperty>
    


    <!-- http://library.ucsd.edu/ontology/dams/#subject -->

    <owl:ObjectProperty rdf:about="&ns4;#subject">
        <rdfs:label>subject</rdfs:label>
        <rdfs:comment>Links an item to a Subject.</rdfs:comment>
        <rdfs:domain rdf:resource="&ns4;#DAMSResource"/>
        <rdfs:range rdf:resource="&ns4;#Subject"/>
    </owl:ObjectProperty>
    


    <!-- http://library.ucsd.edu/ontology/dams/#subjectPart -->

    <owl:ObjectProperty rdf:about="&ns4;#subjectPart">
        <rdfs:label>subjectPart</rdfs:label>
        <rdfs:comment>Links a Subject to a SubjectPart</rdfs:comment>
        <rdfs:domain rdf:resource="&ns4;#Subject"/>
        <rdfs:range rdf:resource="&ns4;#SubjectPart"/>
    </owl:ObjectProperty>
    


    <!-- http://library.ucsd.edu/ontology/dams/#title -->

    <owl:ObjectProperty rdf:about="&ns4;#title">
        <rdfs:comment>Links from a metadata record to a Title.</rdfs:comment>
        <rdfs:range rdf:resource="&ns4;#Title"/>
        <rdfs:domain>
            <owl:Class>
                <owl:unionOf rdf:parseType="Collection">
                    <rdf:Description rdf:about="&ns4;#DAMSResource"/>
                    <rdf:Description rdf:about="&ns4;#Subject"/>
                </owl:unionOf>
            </owl:Class>
        </rdfs:domain>
    </owl:ObjectProperty>
    


    <!-- http://library.ucsd.edu/ontology/dams/#vocabulary -->

    <owl:ObjectProperty rdf:about="&ns4;#vocabulary">
        <rdfs:comment>Links a VocabularyEntry to the Vocabulary that contains it.</rdfs:comment>
        <rdfs:range rdf:resource="&ns4;#Vocabulary"/>
        <rdfs:domain rdf:resource="&ns4;#VocabularyEntry"/>
    </owl:ObjectProperty>
    


    <!-- 
    ///////////////////////////////////////////////////////////////////////////////////////
    //
    // Data properties
    //
    ///////////////////////////////////////////////////////////////////////////////////////
     -->

    


    <!-- http://library.ucsd.edu/ontology/dams/#authority -->

    <owl:DatatypeProperty rdf:about="&ns4;#authority">
        <rdfs:label>authority</rdfs:label>
        <rdfs:comment>Name of controlled vocabulary or other authority for a given metadata element.</rdfs:comment>
        <rdfs:domain rdf:resource="&ns4;#Title"/>
        <rdfs:domain rdf:resource="&ns4;#VocabularyEntry"/>
        <rdfs:range rdf:resource="&xsd;string"/>
    </owl:DatatypeProperty>
    


    <!-- http://library.ucsd.edu/ontology/dams/#authorityURI -->

    <owl:DatatypeProperty rdf:about="&ns4;#authorityURI">
        <rdfs:comment>URI identifying the authority used for a given metadata element, typically used
      when a valueURI is not available.</rdfs:comment>
        <rdfs:range rdf:resource="&xsd;anyURI"/>
    </owl:DatatypeProperty>
    


    <!-- http://library.ucsd.edu/ontology/dams/#beginDate -->

    <owl:DatatypeProperty rdf:about="&ns4;#beginDate">
        <rdfs:label>beginDate</rdfs:label>
        <rdfs:comment>The date when the date range started (ISO 8601).</rdfs:comment>
        <rdfs:domain rdf:resource="&ns4;#Date"/>
        <rdfs:range rdf:resource="&xsd;dateTime"/>
    </owl:DatatypeProperty>
    


    <!-- http://library.ucsd.edu/ontology/dams/#captureSource -->

    <owl:DatatypeProperty rdf:about="&ns4;#captureSource">
        <rdfs:comment>Type of device used to scan an image.</rdfs:comment>
        <rdfs:domain rdf:resource="&ns4;#SourceCapture"/>
    </owl:DatatypeProperty>
    


    <!-- http://library.ucsd.edu/ontology/dams/#checksum -->

    <owl:DatatypeProperty rdf:about="&ns4;#checksum">
        <rdfs:label>checksum</rdfs:label>
        <rdfs:comment>Records the Checksum of a File.</rdfs:comment>
        <rdfs:domain rdf:resource="&ns4;#File"/>
        <rdfs:range rdf:resource="&xsd;hexBinary"/>
    </owl:DatatypeProperty>
    


    <!-- http://library.ucsd.edu/ontology/dams/#code -->

    <owl:DatatypeProperty rdf:about="&ns4;#code"/>
    


    <!-- http://library.ucsd.edu/ontology/dams/#compositionLevel -->

    <owl:DatatypeProperty rdf:about="&ns4;#compositionLevel">
        <rdfs:comment>Decoding/unbundling steps required to extract file. Neccessary?</rdfs:comment>
        <rdfs:domain rdf:resource="&ns4;#File"/>
        <rdfs:range rdf:resource="&xsd;integer"/>
    </owl:DatatypeProperty>
    


    <!-- http://library.ucsd.edu/ontology/dams/#copyrightJurisdiction -->

    <owl:DatatypeProperty rdf:about="&ns4;#copyrightJurisdiction">
        <rdfs:comment>An indication of the legal jurisdiction (typically national) in with the
      copyright status statement is true (ISO 3166-1)</rdfs:comment>
        <rdfs:domain rdf:resource="&ns4;#Copyright"/>
    </owl:DatatypeProperty>
    


    <!-- http://library.ucsd.edu/ontology/dams/#copyrightNote -->

    <owl:DatatypeProperty rdf:about="&ns4;#copyrightNote">
        <rdfs:comment>boilerplate copyright note referencing copyright status and jurisdiction.</rdfs:comment>
        <rdfs:comment>Estimate that there will be 6 of these Note objects.</rdfs:comment>
        <rdfs:domain rdf:resource="&ns4;#Copyright"/>
    </owl:DatatypeProperty>
    


    <!-- http://library.ucsd.edu/ontology/dams/#copyrightStatus -->

    <owl:DatatypeProperty rdf:about="&ns4;#copyrightStatus">
        <rdfs:comment>In context of UCSD, &quot;Under copyright -- 1st Party&quot; refers always and
      only to &quot;UC Regents&quot; as the rights holder, whereas &quot;Under copyright -- 3rd
      party&quot; refers to copyright held by any agent other than the UC Regents.</rdfs:comment>
        <rdfs:comment>An value indicating the copyright status for an object</rdfs:comment>
        <rdfs:domain rdf:resource="&ns4;#Copyright"/>
    </owl:DatatypeProperty>
    


    <!-- http://library.ucsd.edu/ontology/dams/#crc32checksum -->

    <owl:DatatypeProperty rdf:about="&ns4;#crc32checksum">
        <rdfs:comment>Checksum calculated using the CRC32 algorithm.</rdfs:comment>
        <rdfs:domain rdf:resource="&ns4;#File"/>
        <rdfs:subPropertyOf rdf:resource="&ns4;#checksum"/>
        <rdfs:range rdf:resource="&xsd;hexBinary"/>
    </owl:DatatypeProperty>
    


    <!-- http://library.ucsd.edu/ontology/dams/#dateCreatedByApplication -->

    <owl:DatatypeProperty rdf:about="&ns4;#dateCreatedByApplication">
        <rdfs:comment>Date and time the file was created. (ISO 8601)</rdfs:comment>
        <rdfs:domain rdf:resource="&ns4;#File"/>
        <rdfs:range rdf:resource="&xsd;dateTime"/>
    </owl:DatatypeProperty>
    


    <!-- http://library.ucsd.edu/ontology/dams/#description -->

    <owl:DatatypeProperty rdf:about="&ns4;#description">
        <rdfs:label>description</rdfs:label>
        <rdfs:comment>Basic description.</rdfs:comment>
        <rdfs:range rdf:resource="&xsd;string"/>
    </owl:DatatypeProperty>
    


    <!-- http://library.ucsd.edu/ontology/dams/#detail -->

    <owl:DatatypeProperty rdf:about="&ns4;#detail">
        <rdfs:label>detail</rdfs:label>
        <rdfs:comment>Description of the event, containing any relevant details.</rdfs:comment>
        <rdfs:domain rdf:resource="&ns4;#DAMSEvent"/>
        <rdfs:range rdf:resource="&xsd;string"/>
    </owl:DatatypeProperty>
    


    <!-- http://library.ucsd.edu/ontology/dams/#displayLabel -->

    <owl:DatatypeProperty rdf:about="&ns4;#displayLabel">
        <rdfs:comment>User display value.  If the source vocabulary contains both coded and
      human-readable forms, use the human-readable form here.</rdfs:comment>
        <rdfs:range rdf:resource="&xsd;string"/>
    </owl:DatatypeProperty>
    


    <!-- http://library.ucsd.edu/ontology/dams/#encoding -->

    <owl:DatatypeProperty rdf:about="&ns4;#encoding">
        <rdfs:comment>Encoding used for date values (could be implemented as typed literals or
      separate property).</rdfs:comment>
        <rdfs:domain rdf:resource="&ns4;#Date"/>
        <rdfs:range>
            <rdfs:Datatype>
                <owl:oneOf>
                    <rdf:Description>
                        <rdf:type rdf:resource="&rdf;List"/>
                        <rdf:first rdf:datatype="&xsd;string">ISO 8601</rdf:first>
                        <rdf:rest rdf:resource="&rdf;nil"/>
                    </rdf:Description>
                </owl:oneOf>
            </rdfs:Datatype>
        </rdfs:range>
    </owl:DatatypeProperty>
    


    <!-- http://library.ucsd.edu/ontology/dams/#endDate -->

    <owl:DatatypeProperty rdf:about="&ns4;#endDate">
        <rdfs:label>endDate</rdfs:label>
        <rdfs:comment>Date when the date range or event finished (ISO 8601).</rdfs:comment>
        <rdfs:domain rdf:resource="&ns4;#DAMSEvent"/>
        <rdfs:domain rdf:resource="&ns4;#Date"/>
        <rdfs:range rdf:resource="&xsd;dateTime"/>
    </owl:DatatypeProperty>
    


    <!-- http://library.ucsd.edu/ontology/dams/#expression -->

    <owl:DatatypeProperty rdf:about="&ns4;#expression">
        <rdfs:label>expression</rdfs:label>
        <rdfs:comment>Text form of a date, which does not necessarily correspond to a specific numeric
      date (e.g., &quot;Easter&quot;).</rdfs:comment>
        <rdfs:domain rdf:resource="&ns4;#Date"/>
        <rdfs:range rdf:resource="&xsd;string"/>
    </owl:DatatypeProperty>
    


    <!-- http://library.ucsd.edu/ontology/dams/#formatName -->

    <owl:DatatypeProperty rdf:about="&ns4;#formatName">
        <rdfs:comment>Name of the file format (MIME type).</rdfs:comment>
        <rdfs:domain rdf:resource="&ns4;#File"/>
        <rdfs:range rdf:resource="&xsd;string"/>
    </owl:DatatypeProperty>
    


    <!-- http://library.ucsd.edu/ontology/dams/#formatVersion -->

    <owl:DatatypeProperty rdf:about="&ns4;#formatVersion">
        <rdfs:comment>Version of the format in formatName (6.0, 2003, etc.)</rdfs:comment>
        <rdfs:domain rdf:resource="&ns4;#File"/>
        <rdfs:range rdf:resource="&xsd;string"/>
    </owl:DatatypeProperty>
    


    <!-- http://library.ucsd.edu/ontology/dams/#imageProducer -->

    <owl:DatatypeProperty rdf:about="&ns4;#imageProducer">
        <rdfs:comment>Organization that scanned an image.</rdfs:comment>
        <rdfs:domain rdf:resource="&ns4;#SourceCapture"/>
    </owl:DatatypeProperty>
    


    <!-- http://library.ucsd.edu/ontology/dams/#internalOnly -->

    <owl:DatatypeProperty rdf:about="&ns4;#internalOnly">
        <rdfs:comment>If true, accessible to all users or only to repository and DAMS managers.</rdfs:comment>
        <rdfs:comment>false = public, true = custodial repository</rdfs:comment>
        <rdfs:domain rdf:resource="&ns4;#Note"/>
        <rdfs:range rdf:resource="&xsd;boolean"/>
    </owl:DatatypeProperty>
    


    <!-- http://library.ucsd.edu/ontology/dams/#label -->

    <owl:DatatypeProperty rdf:about="&ns4;#label">
        <rdfs:comment>Label describing a component; can be a literal or URI referencing a Title or Date.</rdfs:comment>
        <rdfs:domain rdf:resource="&ns4;#Component"/>
        <rdfs:range rdf:resource="&xsd;string"/>
    </owl:DatatypeProperty>
    


    <!-- http://library.ucsd.edu/ontology/dams/#licenseNote -->

    <owl:DatatypeProperty rdf:about="&ns4;#licenseNote">
        <rdfs:comment>Summary of a license and its terms, either in place of a license or as an
      abstract on a license linked to.</rdfs:comment>
        <rdfs:domain rdf:resource="&ns4;#License"/>
    </owl:DatatypeProperty>
    


    <!-- http://library.ucsd.edu/ontology/dams/#licenseURI -->

    <owl:DatatypeProperty rdf:about="&ns4;#licenseURI">
        <rdfs:comment>Actionable link to a license document or terms.</rdfs:comment>
        <rdfs:domain rdf:resource="&ns4;#License"/>
        <rdfs:range rdf:resource="&xsd;anyURI"/>
    </owl:DatatypeProperty>
    


    <!-- http://library.ucsd.edu/ontology/dams/#line -->

    <owl:DatatypeProperty rdf:about="&ns4;#line">
        <rdfs:comment>Coordinates for a line (last point is not assumed to link to the first
      point)</rdfs:comment>
        <rdfs:comment>Need content standard for data being entered (delimiters between lat, long and
      alt and between coordinate sets).</rdfs:comment>
        <rdfs:domain rdf:resource="&ns4;#Cartographics"/>
    </owl:DatatypeProperty>
    


    <!-- http://library.ucsd.edu/ontology/dams/#md5checksum -->

    <owl:DatatypeProperty rdf:about="&ns4;#md5checksum">
        <rdfs:comment>Checksum calculated using the MD5 algorithm.</rdfs:comment>
        <rdfs:domain rdf:resource="&ns4;#File"/>
        <rdfs:subPropertyOf rdf:resource="&ns4;#checksum"/>
        <rdfs:range rdf:resource="&xsd;hexBinary"/>
    </owl:DatatypeProperty>
    


    <!-- http://library.ucsd.edu/ontology/dams/#nonsortCharacters -->

    <owl:DatatypeProperty rdf:about="&ns4;#nonsortCharacters">
        <rdfs:comment>Initial characters which should not affect sort order.</rdfs:comment>
        <rdfs:comment>Included to facilitate generating sort form without having to build complex
      algorithm to handle multiple languages.</rdfs:comment>
        <rdfs:domain rdf:resource="&ns4;#Title"/>
        <rdfs:range rdf:resource="&xsd;string"/>
    </owl:DatatypeProperty>
    


    <!-- http://library.ucsd.edu/ontology/dams/#objectCategory -->

    <owl:DatatypeProperty rdf:about="&ns4;#objectCategory">
        <rdfs:comment>Whether the entity is a bitstream, file or object.  Neccessary?</rdfs:comment>
        <rdfs:domain rdf:resource="&ns4;#File"/>
        <rdfs:range>
            <rdfs:Datatype>
                <owl:oneOf>
                    <rdf:Description>
                        <rdf:type rdf:resource="&rdf;List"/>
                        <rdf:first rdf:datatype="&xsd;string">file</rdf:first>
                        <rdf:rest rdf:resource="&rdf;nil"/>
                    </rdf:Description>
                </owl:oneOf>
            </rdfs:Datatype>
        </rdfs:range>
    </owl:DatatypeProperty>
    


    <!-- http://library.ucsd.edu/ontology/dams/#order -->

    <owl:DatatypeProperty rdf:about="&ns4;#order">
        <rdfs:comment>Numerical order of the metadata element within the larger grouping.</rdfs:comment>
        <rdfs:range rdf:resource="&xsd;integer"/>
    </owl:DatatypeProperty>
    


    <!-- http://library.ucsd.edu/ontology/dams/#otherRightsBasis -->

    <owl:DatatypeProperty rdf:about="&ns4;#otherRightsBasis">
        <rdfs:comment>For indicating the type or source of the other rights, e.g., UC San Diego
       Policy, UC Policy, etc.</rdfs:comment>
        <rdfs:domain rdf:resource="&ns4;#OtherRights"/>
    </owl:DatatypeProperty>
    


    <!-- http://library.ucsd.edu/ontology/dams/#otherRightsNote -->

    <owl:DatatypeProperty rdf:about="&ns4;#otherRightsNote">
        <rdfs:comment>Summary of institutional policy.</rdfs:comment>
        <rdfs:domain rdf:resource="&ns4;#OtherRights"/>
    </owl:DatatypeProperty>
    


    <!-- http://library.ucsd.edu/ontology/dams/#otherRightsURI -->

    <owl:DatatypeProperty rdf:about="&ns4;#otherRightsURI">
        <rdfs:comment>An actionable link to the documentation containing the institutional policy or
       other rights being applied</rdfs:comment>
        <rdfs:domain rdf:resource="&ns4;#OtherRights"/>
        <rdfs:range rdf:resource="&xsd;anyURI"/>
    </owl:DatatypeProperty>
    


    <!-- http://library.ucsd.edu/ontology/dams/#outcome -->

    <owl:DatatypeProperty rdf:about="&ns4;#outcome">
        <rdfs:comment>Whether the event succeeded or failed.</rdfs:comment>
        <rdfs:domain rdf:resource="&ns4;#DAMSEvent"/>
        <rdfs:range>
            <rdfs:Datatype>
                <owl:oneOf>
                    <rdf:Description>
                        <rdf:type rdf:resource="&rdf;List"/>
                        <rdf:first rdf:datatype="&xsd;string">&#39;Action succeeded&#39;, &#39;Action failed&#39;</rdf:first>
                        <rdf:rest rdf:resource="&rdf;nil"/>
                    </rdf:Description>
                </owl:oneOf>
            </rdfs:Datatype>
        </rdfs:range>
    </owl:DatatypeProperty>
    


    <!-- http://library.ucsd.edu/ontology/dams/#outcomeNote -->

    <owl:DatatypeProperty rdf:about="&ns4;#outcomeNote">
        <rdfs:comment>Extended information about the event, including any relevant status message
      and timestamp.</rdfs:comment>
        <rdfs:domain rdf:resource="&ns4;#DAMSEvent"/>
        <rdfs:range rdf:resource="&xsd;string"/>
    </owl:DatatypeProperty>
    


    <!-- http://library.ucsd.edu/ontology/dams/#partName -->

    <owl:DatatypeProperty rdf:about="&ns4;#partName">
        <rdfs:label>partName</rdfs:label>
        <rdfs:comment>Volume, issue, etc. name.</rdfs:comment>
        <rdfs:domain rdf:resource="&ns4;#Title"/>
        <rdfs:range rdf:resource="&xsd;string"/>
    </owl:DatatypeProperty>
    


    <!-- http://library.ucsd.edu/ontology/dams/#partNumber -->

    <owl:DatatypeProperty rdf:about="&ns4;#partNumber">
        <rdfs:label>partNumber</rdfs:label>
        <rdfs:comment>Volume, issue, etc. number.</rdfs:comment>
        <rdfs:domain rdf:resource="&ns4;#Title"/>
        <rdfs:range rdf:resource="&xsd;string"/>
    </owl:DatatypeProperty>
    


    <!-- http://library.ucsd.edu/ontology/dams/#point -->

    <owl:DatatypeProperty rdf:about="&ns4;#point">
        <rdfs:comment>Coordinates for a single point.</rdfs:comment>
        <rdfs:comment>Need content standard for data being entered (delimiters between lat, long and
      alt and between coordinate sets).</rdfs:comment>
        <rdfs:domain rdf:resource="&ns4;#Cartographics"/>
    </owl:DatatypeProperty>
    


    <!-- http://library.ucsd.edu/ontology/dams/#polygon -->

    <owl:DatatypeProperty rdf:about="&ns4;#polygon">
        <rdfs:comment>Need content standard for data being entered (delimiters between lat, long and
      alt and between coordinate sets).</rdfs:comment>
        <rdfs:comment>Coordinates for a polygon (last point is assumed to link to the first point to
      form an enclosed area).</rdfs:comment>
        <rdfs:domain rdf:resource="&ns4;#Cartographics"/>
    </owl:DatatypeProperty>
    


    <!-- http://library.ucsd.edu/ontology/dams/#preservationLevel -->

    <owl:DatatypeProperty rdf:about="&ns4;#preservationLevel">
        <rdfs:comment>Level of preservation of the file (bit-level, full, 0, 1, 2, fully supported
      with future migrations).  Neccessary?</rdfs:comment>
        <rdfs:domain rdf:resource="&ns4;#File"/>
        <rdfs:range>
            <rdfs:Datatype>
                <owl:oneOf>
                    <rdf:Description>
                        <rdf:type rdf:resource="&rdf;List"/>
                        <rdf:first rdf:datatype="&xsd;string">&#39;bit-level&#39;, &#39;full&#39;, &#39;0&#39;, &#39;1&#39;, &#39;2&#39;</rdf:first>
                        <rdf:rest rdf:resource="&rdf;nil"/>
                    </rdf:Description>
                </owl:oneOf>
            </rdfs:Datatype>
        </rdfs:range>
    </owl:DatatypeProperty>
    


    <!-- http://library.ucsd.edu/ontology/dams/#projection -->

    <owl:DatatypeProperty rdf:about="&ns4;#projection">
        <rdfs:comment>See http://en.wikipedia.org/wiki/List_of_map_projections</rdfs:comment>
        <rdfs:comment>The method of representing the surface of a sphere or other three-dimensional
      body on a plane.</rdfs:comment>
        <rdfs:domain rdf:resource="&ns4;#Cartographics"/>
    </owl:DatatypeProperty>
    


    <!-- http://library.ucsd.edu/ontology/dams/#purposeNote -->

    <owl:DatatypeProperty rdf:about="&ns4;#purposeNote">
        <rdfs:comment>boilerplate text stating the content is made available for educational
      purposes.</rdfs:comment>
        <rdfs:domain rdf:resource="&ns4;#Copyright"/>
    </owl:DatatypeProperty>
    


    <!-- http://library.ucsd.edu/ontology/dams/#referenceSystem -->

    <owl:DatatypeProperty rdf:about="&ns4;#referenceSystem">
        <rdfs:comment>The standard coordinate frame for the coordinates being used (WGS66, WGS72,
      WGS84).</rdfs:comment>
        <rdfs:domain rdf:resource="&ns4;#Cartographics"/>
    </owl:DatatypeProperty>
    


    <!-- http://library.ucsd.edu/ontology/dams/#repositoryName -->

    <owl:DatatypeProperty rdf:about="&ns4;#repositoryName">
        <rdfs:comment>The name of the repository or organizational unit assuming custodial
      responsibility for DAMS content.</rdfs:comment>
        <rdfs:domain rdf:resource="&ns4;#Repository"/>
        <rdfs:range rdf:resource="&xsd;string"/>
    </owl:DatatypeProperty>
    


    <!-- http://library.ucsd.edu/ontology/dams/#repositoryURI -->

    <owl:DatatypeProperty rdf:about="&ns4;#repositoryURI">
        <rdfs:comment>The URI linking to a webpage for the repository that contains contact and
      access information about the repository.</rdfs:comment>
        <rdfs:domain rdf:resource="&ns4;#Repository"/>
        <rdfs:range rdf:resource="&xsd;string"/>
    </owl:DatatypeProperty>
    


    <!-- http://library.ucsd.edu/ontology/dams/#scale -->

    <owl:DatatypeProperty rdf:about="&ns4;#scale">
        <rdfs:comment>The relative size of the representation or rendering of geographic information
      (i.e. map, chart, model) to the actual location.</rdfs:comment>
        <rdfs:domain rdf:resource="&ns4;#Cartographics"/>
    </owl:DatatypeProperty>
    


    <!-- http://library.ucsd.edu/ontology/dams/#scannerManufacturer -->

    <owl:DatatypeProperty rdf:about="&ns4;#scannerManufacturer">
        <rdfs:comment>Manufacturer of the scanner used to scan an image.</rdfs:comment>
        <rdfs:domain rdf:resource="&ns4;#SourceCapture"/>
    </owl:DatatypeProperty>
    


    <!-- http://library.ucsd.edu/ontology/dams/#scannerModelName -->

    <owl:DatatypeProperty rdf:about="&ns4;#scannerModelName">
        <rdfs:comment>Model name of the scanner used to scan an image.</rdfs:comment>
        <rdfs:domain rdf:resource="&ns4;#SourceCapture"/>
    </owl:DatatypeProperty>
    


    <!-- http://library.ucsd.edu/ontology/dams/#scanningSoftware -->

    <owl:DatatypeProperty rdf:about="&ns4;#scanningSoftware">
        <rdfs:comment>Name of the software application used to scan an image.</rdfs:comment>
        <rdfs:domain rdf:resource="&ns4;#SourceCapture"/>
    </owl:DatatypeProperty>
    


    <!-- http://library.ucsd.edu/ontology/dams/#scanningSoftwareVersion -->

    <owl:DatatypeProperty rdf:about="&ns4;#scanningSoftwareVersion">
        <rdfs:comment>Version number of the software used to scan an image.</rdfs:comment>
        <rdfs:domain rdf:resource="&ns4;#SourceCapture"/>
    </owl:DatatypeProperty>
    


    <!-- http://library.ucsd.edu/ontology/dams/#script -->

    <owl:DatatypeProperty rdf:about="&ns4;#script">
        <rdfs:comment>Writing system used for a given metadata element.</rdfs:comment>
        <rdfs:domain rdf:resource="&ns4;#Title"/>
        <rdfs:range rdf:resource="&xsd;string"/>
    </owl:DatatypeProperty>
    


    <!-- http://library.ucsd.edu/ontology/dams/#sha1checksum -->

    <owl:DatatypeProperty rdf:about="&ns4;#sha1checksum">
        <rdfs:label>sha1checksum</rdfs:label>
        <rdfs:comment>Checksum calculated using the SHA-1 algorithm.</rdfs:comment>
        <rdfs:domain rdf:resource="&ns4;#File"/>
        <rdfs:subPropertyOf rdf:resource="&ns4;#checksum"/>
        <rdfs:range rdf:resource="&xsd;hexBinary"/>
    </owl:DatatypeProperty>
    


    <!-- http://library.ucsd.edu/ontology/dams/#sha256checksum -->

    <owl:DatatypeProperty rdf:about="&ns4;#sha256checksum">
        <rdfs:label>sha256checksum</rdfs:label>
        <rdfs:comment>Checksum calculated using the SHA-256 algorithm.</rdfs:comment>
        <rdfs:domain rdf:resource="&ns4;#File"/>
        <rdfs:subPropertyOf rdf:resource="&ns4;#checksum"/>
        <rdfs:range rdf:resource="&xsd;hexBinary"/>
    </owl:DatatypeProperty>
    


    <!-- http://library.ucsd.edu/ontology/dams/#sha512checksum -->

    <owl:DatatypeProperty rdf:about="&ns4;#sha512checksum">
        <rdfs:label>sha512checksum</rdfs:label>
        <rdfs:comment>Checksum calculated using the SHA-512 algorithm.</rdfs:comment>
        <rdfs:domain rdf:resource="&ns4;#File"/>
        <rdfs:subPropertyOf rdf:resource="&ns4;#checksum"/>
        <rdfs:range rdf:resource="&xsd;hexBinary"/>
    </owl:DatatypeProperty>
    


    <!-- http://library.ucsd.edu/ontology/dams/#size -->

    <owl:DatatypeProperty rdf:about="&ns4;#size">
        <rdfs:label>size</rdfs:label>
        <rdfs:comment>Size of the file in bytes.</rdfs:comment>
        <rdfs:domain rdf:resource="&ns4;#File"/>
        <rdfs:range rdf:resource="&xsd;integer"/>
    </owl:DatatypeProperty>
    


    <!-- http://library.ucsd.edu/ontology/dams/#sourceType -->

    <owl:DatatypeProperty rdf:about="&ns4;#sourceType">
        <rdfs:comment>The medium of the analog source material scanned to create an
      image.</rdfs:comment>
        <rdfs:domain rdf:resource="&ns4;#SourceCapture"/>
    </owl:DatatypeProperty>
    


    <!-- http://library.ucsd.edu/ontology/dams/#statuteCitation -->

    <owl:DatatypeProperty rdf:about="&ns4;#statuteCitation">
        <rdfs:comment>The name of the statute, e.g., Family Education Rights and Privacy Act
      (FERPA)</rdfs:comment>
        <rdfs:domain rdf:resource="&ns4;#Statute"/>
    </owl:DatatypeProperty>
    


    <!-- http://library.ucsd.edu/ontology/dams/#statuteJurisdiction -->

    <owl:DatatypeProperty rdf:about="&ns4;#statuteJurisdiction">
        <rdfs:comment>The country or regional jurisdiction in which the statute applies (ISO 3166-1
      for country codes, ISO 3166-2 for state codes).</rdfs:comment>
        <rdfs:domain rdf:resource="&ns4;#Statute"/>
    </owl:DatatypeProperty>
    


    <!-- http://library.ucsd.edu/ontology/dams/#statuteNote -->

    <owl:DatatypeProperty rdf:about="&ns4;#statuteNote">
        <rdfs:comment>Summary of a statute and obligation to it, e.g., students records must be
      restricted for 50 years after creation or death (or whatever the actual terms are
      now)</rdfs:comment>
        <rdfs:domain rdf:resource="&ns4;#Statute"/>
    </owl:DatatypeProperty>
    


    <!-- http://library.ucsd.edu/ontology/dams/#subtitle -->

    <owl:DatatypeProperty rdf:about="&ns4;#subtitle">
        <rdfs:label>subtitle</rdfs:label>
        <rdfs:comment>Explanatory or alternate title.</rdfs:comment>
        <rdfs:domain rdf:resource="&ns4;#Title"/>
        <rdfs:range rdf:resource="&xsd;string"/>
    </owl:DatatypeProperty>
    


    <!-- http://library.ucsd.edu/ontology/dams/#term -->

    <owl:DatatypeProperty rdf:about="&ns4;#term">
        <rdfs:label>term</rdfs:label>
        <rdfs:comment>Actionable term name.  If the source vocabulary contains both coded and
      human-readable forms, use the coded form here.</rdfs:comment>
        <rdfs:domain rdf:resource="&ns4;#VocabularyEntry"/>
        <rdfs:range rdf:resource="&xsd;string"/>
    </owl:DatatypeProperty>
    


    <!-- http://library.ucsd.edu/ontology/dams/#type -->

    <owl:DatatypeProperty rdf:about="&ns4;#type">
        <rdfs:label>type</rdfs:label>
        <rdfs:comment>Qualifier of a metadata element to differentiate different kinds of values.</rdfs:comment>
        <rdfs:range rdf:resource="&xsd;string"/>
    </owl:DatatypeProperty>
    


    <!-- http://library.ucsd.edu/ontology/dams/#uri -->

    <owl:DatatypeProperty rdf:about="&ns4;#uri">
        <rdfs:comment>URI where the related resource can be accessed.  In the case of internal links,
      a DAMS URI should be used.</rdfs:comment>
        <rdfs:domain rdf:resource="&ns4;#RelatedResource"/>
        <rdfs:range rdf:resource="&xsd;anyURI"/>
    </owl:DatatypeProperty>
    


    <!-- http://library.ucsd.edu/ontology/dams/#use -->

    <owl:DatatypeProperty rdf:about="&ns4;#use">
        <rdfs:comment>Type of file and its role to the object.</rdfs:comment>
        <rdfs:domain rdf:resource="&ns4;#File"/>
        <rdfs:range>
            <rdfs:Datatype>
                <owl:oneOf>
                    <rdf:Description>
                        <rdf:type rdf:resource="&rdf;List"/>
                        <rdf:first rdf:datatype="&xsd;string">&#39;visual-source&#39;, &#39;visual-service&#39;, &#39;visual-thumbnail&#39;, &#39;visual-alternate&#39;, &#39;document-source&#39;, &#39;document-service&#39;, &#39;document-alternate&#39;, &#39;audio-source&#39;, &#39;audio-service&#39;, &#39;audio-alternate&#39;, &#39;data-source&#39;, &#39;data-service&#39;, &#39;data-alternate&#39;</rdf:first>
                        <rdf:rest rdf:resource="&rdf;nil"/>
                    </rdf:Description>
                </owl:oneOf>
            </rdfs:Datatype>
        </rdfs:range>
    </owl:DatatypeProperty>
    


    <!-- http://library.ucsd.edu/ontology/dams/#value -->

    <owl:DatatypeProperty rdf:about="&ns4;#value">
        <rdfs:label>value</rdfs:label>
        <rdfs:comment>Primary value of a metadata element.</rdfs:comment>
        <rdfs:range rdf:resource="&xsd;string"/>
    </owl:DatatypeProperty>
    


    <!-- http://library.ucsd.edu/ontology/dams/#valueURI -->

    <owl:DatatypeProperty rdf:about="&ns4;#valueURI">
        <rdfs:comment>URI uniquely identifying the term used for a given metadata element.</rdfs:comment>
        <rdfs:range rdf:resource="&xsd;anyURI"/>
    </owl:DatatypeProperty>
    


    <!-- 
    ///////////////////////////////////////////////////////////////////////////////////////
    //
    // Classes
    //
    ///////////////////////////////////////////////////////////////////////////////////////
     -->

    


    <!-- http://library.ucsd.edu/ontology/dams/ProvenanceCollection -->

    <owl:Class rdf:about="&ns4;ProvenanceCollection">
        <rdfs:subClassOf rdf:resource="&ns4;#Collection"/>
        <rdfs:subClassOf>
            <owl:Restriction>
                <owl:onProperty rdf:resource="&ns4;#hasCollection"/>
                <owl:cardinality rdf:datatype="&xsd;nonNegativeInteger">0</owl:cardinality>
            </owl:Restriction>
        </rdfs:subClassOf>
        <rdfs:subClassOf>
            <owl:Restriction>
                <owl:onProperty rdf:resource="&ns4;#hasPart"/>
                <owl:allValuesFrom rdf:resource="&ns4;ProvenanceCollectionPart"/>
            </owl:Restriction>
        </rdfs:subClassOf>
        <rdfs:subClassOf>
            <owl:Restriction>
                <owl:onProperty rdf:resource="&ns4;#hasProvenanceCollection"/>
                <owl:cardinality rdf:datatype="&xsd;nonNegativeInteger">0</owl:cardinality>
            </owl:Restriction>
        </rdfs:subClassOf>
    </owl:Class>
    


    <!-- http://library.ucsd.edu/ontology/dams/ProvenanceCollectionPart -->

    <owl:Class rdf:about="&ns4;ProvenanceCollectionPart">
        <rdfs:subClassOf rdf:resource="&ns4;#Collection"/>
        <rdfs:subClassOf>
            <owl:Restriction>
                <owl:onProperty rdf:resource="&ns4;#hasCollection"/>
                <owl:cardinality rdf:datatype="&xsd;nonNegativeInteger">0</owl:cardinality>
            </owl:Restriction>
        </rdfs:subClassOf>
        <rdfs:subClassOf>
            <owl:Restriction>
                <owl:onProperty rdf:resource="&ns4;#provenanceCollection"/>
                <owl:onClass rdf:resource="&ns4;ProvenanceCollection"/>
                <owl:qualifiedCardinality rdf:datatype="&xsd;nonNegativeInteger">1</owl:qualifiedCardinality>
            </owl:Restriction>
        </rdfs:subClassOf>
        <rdfs:subClassOf>
            <owl:Restriction>
                <owl:onProperty rdf:resource="&ns4;#hasProvenanceCollection"/>
                <owl:cardinality rdf:datatype="&xsd;nonNegativeInteger">0</owl:cardinality>
            </owl:Restriction>
        </rdfs:subClassOf>
    </owl:Class>
    


    <!-- http://library.ucsd.edu/ontology/dams/#Cartographics -->

    <owl:Class rdf:about="&ns4;#Cartographics">
        <rdfs:subClassOf rdf:resource="&ns4;#DAMSThing"/>
        <rdfs:subClassOf>
            <owl:Restriction>
                <owl:onProperty rdf:resource="&ns4;#scale"/>
                <owl:maxQualifiedCardinality rdf:datatype="&xsd;nonNegativeInteger">1</owl:maxQualifiedCardinality>
                <owl:onDataRange rdf:resource="&xsd;string"/>
            </owl:Restriction>
        </rdfs:subClassOf>
        <rdfs:subClassOf>
            <owl:Restriction>
                <owl:onProperty rdf:resource="&ns4;#line"/>
                <owl:maxQualifiedCardinality rdf:datatype="&xsd;nonNegativeInteger">1</owl:maxQualifiedCardinality>
                <owl:onDataRange rdf:resource="&xsd;string"/>
            </owl:Restriction>
        </rdfs:subClassOf>
        <rdfs:subClassOf>
            <owl:Restriction>
                <owl:onProperty rdf:resource="&ns4;#referenceSystem"/>
                <owl:allValuesFrom>
                    <rdfs:Datatype>
                        <owl:oneOf>
                            <rdf:Description>
                                <rdf:type rdf:resource="&rdf;List"/>
                                <rdf:first rdf:datatype="&xsd;string">&#39;WGS84&#39;, &#39;WGS72&#39;, &#39;WGS66&#39;</rdf:first>
                                <rdf:rest rdf:resource="&rdf;nil"/>
                            </rdf:Description>
                        </owl:oneOf>
                    </rdfs:Datatype>
                </owl:allValuesFrom>
            </owl:Restriction>
        </rdfs:subClassOf>
        <rdfs:subClassOf>
            <owl:Restriction>
                <owl:onProperty rdf:resource="&ns4;#polygon"/>
                <owl:maxQualifiedCardinality rdf:datatype="&xsd;nonNegativeInteger">1</owl:maxQualifiedCardinality>
                <owl:onDataRange rdf:resource="&xsd;string"/>
            </owl:Restriction>
        </rdfs:subClassOf>
        <rdfs:subClassOf>
            <owl:Restriction>
                <owl:onProperty rdf:resource="&ns4;#projection"/>
                <owl:maxQualifiedCardinality rdf:datatype="&xsd;nonNegativeInteger">1</owl:maxQualifiedCardinality>
                <owl:onDataRange rdf:resource="&xsd;string"/>
            </owl:Restriction>
        </rdfs:subClassOf>
        <rdfs:subClassOf>
            <owl:Restriction>
                <owl:onProperty rdf:resource="&ns4;#point"/>
                <owl:maxQualifiedCardinality rdf:datatype="&xsd;nonNegativeInteger">1</owl:maxQualifiedCardinality>
                <owl:onDataRange rdf:resource="&xsd;string"/>
            </owl:Restriction>
        </rdfs:subClassOf>
        <rdfs:comment>Information about geographic location (coordinates) or about a representation
      of geographic information (i.e. map, chart, model) for a collection, object, or object
      component.</rdfs:comment>
    </owl:Class>
    


    <!-- http://library.ucsd.edu/ontology/dams/#Collection -->

    <owl:Class rdf:about="&ns4;#Collection">
        <rdfs:label>Collection</rdfs:label>
        <rdfs:subClassOf rdf:resource="&ns4;#DAMSResource"/>
        <rdfs:subClassOf>
            <owl:Restriction>
                <owl:onProperty rdf:resource="&ns4;#scopeContentNote"/>
                <owl:onClass rdf:resource="&ns4;#ScopeContentNote"/>
                <owl:minQualifiedCardinality rdf:datatype="&xsd;nonNegativeInteger">1</owl:minQualifiedCardinality>
            </owl:Restriction>
        </rdfs:subClassOf>
        <rdfs:subClassOf>
            <owl:Restriction>
                <owl:onProperty rdf:resource="&ns4;#title"/>
                <owl:onClass rdf:resource="&ns4;#Title"/>
                <owl:minQualifiedCardinality rdf:datatype="&xsd;nonNegativeInteger">1</owl:minQualifiedCardinality>
            </owl:Restriction>
        </rdfs:subClassOf>
        <rdfs:subClassOf>
            <owl:Restriction>
                <owl:onProperty rdf:resource="&ns4;#hasProvenanceCollection"/>
                <owl:allValuesFrom rdf:resource="&ns4;ProvenanceCollection"/>
            </owl:Restriction>
        </rdfs:subClassOf>
        <rdfs:subClassOf>
            <owl:Restriction>
                <owl:onProperty rdf:resource="&ns4;#collection"/>
                <owl:onClass rdf:resource="&ns4;#Collection"/>
                <owl:maxQualifiedCardinality rdf:datatype="&xsd;nonNegativeInteger">1</owl:maxQualifiedCardinality>
            </owl:Restriction>
        </rdfs:subClassOf>
        <rdfs:subClassOf>
            <owl:Restriction>
                <owl:onProperty rdf:resource="&ns4;#language"/>
                <owl:onClass rdf:resource="&ns4;#Language"/>
                <owl:minQualifiedCardinality rdf:datatype="&xsd;nonNegativeInteger">1</owl:minQualifiedCardinality>
            </owl:Restriction>
        </rdfs:subClassOf>
        <rdfs:comment>Mandatory event: collection record creation.</rdfs:comment>
        <rdfs:comment>Note: only required note is ScopeContentNote</rdfs:comment>
        <rdfs:comment>additional requirements TBD</rdfs:comment>
        <rdfs:comment>An aggregate of objects and/or collections.  One type of
      collection is that in which all members of the collection have the same
      provenance.  A second type of collection is a sub-part of the first type
      but having a title that distinguishes it from the parent collection.  A
      third type of collection is a collection assembled by authorized library
      agents. This collection may be composed on other collections and/or discrete
      objects. Provenance is not a binder for the collection, as the assembled
      collection is typically constructed around a topical facet, e.g. Archive
      for New Poetry, Southworth Spanish Civil War, Melanesian, University Archives,
      etc.</rdfs:comment>
        <rdfs:comment>Collection relationships need to be defined by policy TBD.</rdfs:comment>
        <rdfs:comment>Title and Language: cardinality overrides superclass.</rdfs:comment>
    </owl:Class>
    


    <!-- http://library.ucsd.edu/ontology/dams/#Component -->

    <owl:Class rdf:about="&ns4;#Component">
        <rdfs:label>Component</rdfs:label>
        <rdfs:subClassOf rdf:resource="&ns4;#DAMSResource"/>
        <rdfs:subClassOf>
            <owl:Restriction>
                <owl:onProperty rdf:resource="&ns4;#copyright"/>
                <owl:onClass rdf:resource="&ns4;#Copyright"/>
                <owl:maxQualifiedCardinality rdf:datatype="&xsd;nonNegativeInteger">1</owl:maxQualifiedCardinality>
            </owl:Restriction>
        </rdfs:subClassOf>
        <rdfs:subClassOf>
            <owl:Restriction>
                <owl:onProperty rdf:resource="&ns4;#order"/>
                <owl:qualifiedCardinality rdf:datatype="&xsd;nonNegativeInteger">1</owl:qualifiedCardinality>
                <owl:onDataRange rdf:resource="&xsd;integer"/>
            </owl:Restriction>
        </rdfs:subClassOf>
        <rdfs:subClassOf>
            <owl:Restriction>
                <owl:onProperty rdf:resource="&ns4;#otherRights"/>
                <owl:onClass rdf:resource="&ns4;#OtherRights"/>
                <owl:maxQualifiedCardinality rdf:datatype="&xsd;nonNegativeInteger">1</owl:maxQualifiedCardinality>
            </owl:Restriction>
        </rdfs:subClassOf>
        <rdfs:subClassOf>
            <owl:Restriction>
                <owl:onProperty rdf:resource="&ns4;#statute"/>
                <owl:onClass rdf:resource="&ns4;#Statute"/>
                <owl:maxQualifiedCardinality rdf:datatype="&xsd;nonNegativeInteger">1</owl:maxQualifiedCardinality>
            </owl:Restriction>
        </rdfs:subClassOf>
        <rdfs:subClassOf>
            <owl:Restriction>
                <owl:onProperty rdf:resource="&ns4;#component"/>
                <owl:onClass rdf:resource="&ns4;#Component"/>
                <owl:maxQualifiedCardinality rdf:datatype="&xsd;nonNegativeInteger">1</owl:maxQualifiedCardinality>
            </owl:Restriction>
        </rdfs:subClassOf>
        <rdfs:subClassOf>
            <owl:Restriction>
                <owl:onProperty rdf:resource="&ns4;#license"/>
                <owl:onClass rdf:resource="&ns4;#License"/>
                <owl:maxQualifiedCardinality rdf:datatype="&xsd;nonNegativeInteger">1</owl:maxQualifiedCardinality>
            </owl:Restriction>
        </rdfs:subClassOf>
        <rdfs:subClassOf>
            <owl:Restriction>
                <owl:onProperty rdf:resource="&ns4;#object"/>
                <owl:onClass rdf:resource="&ns4;#Object"/>
                <owl:qualifiedCardinality rdf:datatype="&xsd;nonNegativeInteger">1</owl:qualifiedCardinality>
            </owl:Restriction>
        </rdfs:subClassOf>
        <rdfs:comment>Components are bounded by, unique to an object context and only
      link to other objects having the same object context. Must link to the object
      the component is associated with. If the child of another component, must
      also link to it.</rdfs:comment>
        <rdfs:comment>Mandatory event: component record creation.</rdfs:comment>
        <rdfs:comment>Must have at least one child component or file.</rdfs:comment>
        <rdfs:comment>Must link to parent component if there is one.</rdfs:comment>
        <rdfs:comment>A logical or physical part of an object and contained
      exclusively within the object. The component may consist of metadata and
      one or more content files bound together within the context of the object.
      A component that has no directly associated content files is a logical
      component, whereas a component that has associated content files is a physical
      component. There is no constraint on how many components may occur at any
      given level or how deep the component hierarchy may go.</rdfs:comment>
    </owl:Class>
    


    <!-- http://library.ucsd.edu/ontology/dams/#Copyright -->

    <owl:Class rdf:about="&ns4;#Copyright">
        <rdfs:label>Copyright</rdfs:label>
        <rdfs:subClassOf rdf:resource="&ns4;#Rights"/>
        <rdfs:subClassOf>
            <owl:Restriction>
                <owl:onProperty rdf:resource="&ns4;#copyrightNote"/>
                <owl:allValuesFrom rdf:resource="&xsd;string"/>
            </owl:Restriction>
        </rdfs:subClassOf>
        <rdfs:subClassOf>
            <owl:Restriction>
                <owl:onProperty rdf:resource="&ns4;#rightsAction"/>
                <owl:onClass rdf:resource="&ns4;#RightsAction"/>
                <owl:qualifiedCardinality rdf:datatype="&xsd;nonNegativeInteger">0</owl:qualifiedCardinality>
            </owl:Restriction>
        </rdfs:subClassOf>
        <rdfs:subClassOf>
            <owl:Restriction>
                <owl:onProperty rdf:resource="&ns4;#purposeNote"/>
                <owl:allValuesFrom rdf:resource="&xsd;string"/>
            </owl:Restriction>
        </rdfs:subClassOf>
        <rdfs:subClassOf>
            <owl:Restriction>
                <owl:onProperty rdf:resource="&ns4;#copyrightStatus"/>
                <owl:qualifiedCardinality rdf:datatype="&xsd;nonNegativeInteger">1</owl:qualifiedCardinality>
                <owl:onDataRange>
                    <rdfs:Datatype>
                        <owl:oneOf>
                            <rdf:Description>
                                <rdf:type rdf:resource="&rdf;List"/>
                                <rdf:first rdf:datatype="&xsd;string">&#39;Under copyright -- 1st Party&#39;, &#39;Under copyright -- 3rd Party&#39;, &#39;Public domain&#39;, &#39;Copyright unknown&#39;</rdf:first>
                                <rdf:rest rdf:resource="&rdf;nil"/>
                            </rdf:Description>
                        </owl:oneOf>
                    </rdfs:Datatype>
                </owl:onDataRange>
            </owl:Restriction>
        </rdfs:subClassOf>
        <rdfs:subClassOf>
            <owl:Restriction>
                <owl:onProperty rdf:resource="&ns4;#date"/>
                <owl:onClass rdf:resource="&ns4;#Date"/>
                <owl:maxQualifiedCardinality rdf:datatype="&xsd;nonNegativeInteger">1</owl:maxQualifiedCardinality>
            </owl:Restriction>
        </rdfs:subClassOf>
        <rdfs:subClassOf>
            <owl:Restriction>
                <owl:onProperty rdf:resource="&ns4;#relationship"/>
                <owl:onClass rdf:resource="&ns4;#Relationship"/>
                <owl:maxQualifiedCardinality rdf:datatype="&xsd;nonNegativeInteger">1</owl:maxQualifiedCardinality>
            </owl:Restriction>
        </rdfs:subClassOf>
        <rdfs:subClassOf>
            <owl:Restriction>
                <owl:onProperty rdf:resource="&ns4;#copyrightJurisdiction"/>
                <owl:qualifiedCardinality rdf:datatype="&xsd;nonNegativeInteger">1</owl:qualifiedCardinality>
                <owl:onDataRange rdf:resource="&xsd;string"/>
            </owl:Restriction>
        </rdfs:subClassOf>
        <rdfs:comment>Relationship for Rights Holder.</rdfs:comment>
        <rdfs:comment>The copyright status of an object or object component, indicating if the object
      or object component is under copyright, if it is in the public domain, or if copyright is
      unknown.</rdfs:comment>
    </owl:Class>
    


    <!-- http://library.ucsd.edu/ontology/dams/#CustodialResponsibilityNote -->

    <owl:Class rdf:about="&ns4;#CustodialResponsibilityNote">
        <rdfs:subClassOf rdf:resource="&ns4;#Note"/>
        <rdfs:subClassOf>
            <owl:Restriction>
                <owl:onProperty rdf:resource="&ns4;#type"/>
                <owl:cardinality rdf:datatype="&xsd;nonNegativeInteger">0</owl:cardinality>
            </owl:Restriction>
        </rdfs:subClassOf>
        <rdfs:comment>Note declaring the custodial repository for an object.</rdfs:comment>
        <rdfs:comment>Should be populated by Repository for an object.</rdfs:comment>
    </owl:Class>
    


    <!-- http://library.ucsd.edu/ontology/dams/#DAMSEvent -->

    <owl:Class rdf:about="&ns4;#DAMSEvent">
        <rdfs:subClassOf>
            <owl:Restriction>
                <owl:onProperty rdf:resource="&ns4;#outcome"/>
                <owl:qualifiedCardinality rdf:datatype="&xsd;nonNegativeInteger">1</owl:qualifiedCardinality>
                <owl:onDataRange rdf:resource="&xsd;string"/>
            </owl:Restriction>
        </rdfs:subClassOf>
        <rdfs:subClassOf>
            <owl:Restriction>
                <owl:onProperty rdf:resource="&ns4;#detail"/>
                <owl:minQualifiedCardinality rdf:datatype="&xsd;nonNegativeInteger">1</owl:minQualifiedCardinality>
                <owl:onDataRange rdf:resource="&xsd;string"/>
            </owl:Restriction>
        </rdfs:subClassOf>
        <rdfs:subClassOf>
            <owl:Restriction>
                <owl:onProperty rdf:resource="&ns4;#type"/>
                <owl:qualifiedCardinality rdf:datatype="&xsd;nonNegativeInteger">1</owl:qualifiedCardinality>
                <owl:onDataRange>
                    <rdfs:Datatype>
                        <owl:oneOf>
                            <rdf:Description>
                                <rdf:type rdf:resource="&rdf;List"/>
                                <rdf:first rdf:datatype="&xsd;string">&#39;augmentation--content&#39;, &#39;creation--collection&#39;, &#39;creation--object&#39;, &#39;deletion--object&#39;, &#39;creation--derivative&#39;, &#39;verification--checksum&#39;, &#39;indexing&#39;, &#39;calculation--checksum&#39;, &#39;revision--metadata&#39;, &#39;transformation--metadata&#39;, &#39;migration--content&#39;, &#39;modification--content&#39;, &#39;replication--object&#39;, &#39;validation--object&#39;, &#39;virus check--content&#39;</rdf:first>
                                <rdf:rest rdf:resource="&rdf;nil"/>
                            </rdf:Description>
                        </owl:oneOf>
                    </rdfs:Datatype>
                </owl:onDataRange>
            </owl:Restriction>
        </rdfs:subClassOf>
        <rdfs:subClassOf>
            <owl:Restriction>
                <owl:onProperty rdf:resource="&ns4;#endDate"/>
                <owl:qualifiedCardinality rdf:datatype="&xsd;nonNegativeInteger">1</owl:qualifiedCardinality>
                <owl:onDataRange rdf:resource="&xsd;string"/>
            </owl:Restriction>
        </rdfs:subClassOf>
        <rdfs:subClassOf>
            <owl:Restriction>
                <owl:onProperty rdf:resource="&ns4;#relationship"/>
                <owl:onClass rdf:resource="&ns4;#Relationship"/>
                <owl:minQualifiedCardinality rdf:datatype="&xsd;nonNegativeInteger">1</owl:minQualifiedCardinality>
            </owl:Restriction>
        </rdfs:subClassOf>
        <rdfs:comment>Required name/role: event initiator.</rdfs:comment>
        <rdfs:comment>Any event occurring in the DAMS slated to being tracked. Such events can include
      uploading of content files, creation and updating of metadata records, deletion of objects,
      and transfer of objects and collections to preservation management.</rdfs:comment>
        <rdfs:comment>Ontology: PREMIS</rdfs:comment>
    </owl:Class>
    


    <!-- http://library.ucsd.edu/ontology/dams/#DAMSResource -->

    <owl:Class rdf:about="&ns4;#DAMSResource">
        <rdfs:subClassOf rdf:resource="&ns4;#DAMSThing"/>
        <rdfs:subClassOf>
            <owl:Restriction>
                <owl:onProperty rdf:resource="&ns4;#event"/>
                <owl:onClass rdf:resource="&ns4;#DAMSEvent"/>
                <owl:minQualifiedCardinality rdf:datatype="&xsd;nonNegativeInteger">1</owl:minQualifiedCardinality>
            </owl:Restriction>
        </rdfs:subClassOf>
        <rdfs:comment>Parent of DAMS classes with common descriptive metadata attached (Collection,
      Object, and Component)</rdfs:comment>
        <rdfs:comment>Mandatory event: DAMS Resource creation (collection, object, component).</rdfs:comment>
    </owl:Class>
    


    <!-- http://library.ucsd.edu/ontology/dams/#DAMSThing -->

    <owl:Class rdf:about="&ns4;#DAMSThing">
        <rdfs:subClassOf>
            <owl:Restriction>
                <owl:onProperty rdf:resource="&ns4;#event"/>
                <owl:allValuesFrom rdf:resource="&ns4;#DAMSEvent"/>
            </owl:Restriction>
        </rdfs:subClassOf>
        <rdfs:comment>Parent of all DAMS classes.</rdfs:comment>
    </owl:Class>
    


    <!-- http://library.ucsd.edu/ontology/dams/#Date -->

    <owl:Class rdf:about="&ns4;#Date">
        <rdfs:label>Date</rdfs:label>
        <rdfs:subClassOf rdf:resource="&ns4;#DAMSThing"/>
        <rdfs:subClassOf>
            <owl:Restriction>
                <owl:onProperty rdf:resource="&ns4;#type"/>
                <owl:allValuesFrom>
                    <rdfs:Datatype>
                        <owl:oneOf>
                            <rdf:Description>
                                <rdf:type rdf:resource="&rdf;List"/>
                                <rdf:first rdf:datatype="&xsd;string">&#39;issued&#39;, &#39;created&#39;, &#39;captured&#39;, &#39;valid&#39;, &#39;modified&#39;, &#39;copyright&#39;, &#39;other&#39;</rdf:first>
                                <rdf:rest rdf:resource="&rdf;nil"/>
                            </rdf:Description>
                        </owl:oneOf>
                    </rdfs:Datatype>
                </owl:allValuesFrom>
            </owl:Restriction>
        </rdfs:subClassOf>
        <rdfs:comment>The date(s) for the collection, object, or object component. May be a single date
      or a combination of inclusive dates and/or bulk dates. May indicate if it is the date for
      creation, issuance, capture, copyright, or otherwise.</rdfs:comment>
    </owl:Class>
    


    <!-- http://library.ucsd.edu/ontology/dams/#File -->

    <owl:Class rdf:about="&ns4;#File">
        <rdfs:label>File</rdfs:label>
        <rdfs:subClassOf rdf:resource="&ns4;#DAMSThing"/>
        <rdfs:subClassOf>
            <owl:Restriction>
                <owl:onProperty rdf:resource="&ns4;#component"/>
                <owl:onClass rdf:resource="&ns4;#Component"/>
                <owl:maxQualifiedCardinality rdf:datatype="&xsd;nonNegativeInteger">1</owl:maxQualifiedCardinality>
            </owl:Restriction>
        </rdfs:subClassOf>
        <rdfs:subClassOf>
            <owl:Restriction>
                <owl:onProperty rdf:resource="&ns4;#preservationLevel"/>
                <owl:maxQualifiedCardinality rdf:datatype="&xsd;nonNegativeInteger">1</owl:maxQualifiedCardinality>
                <owl:onDataRange rdf:resource="&xsd;string"/>
            </owl:Restriction>
        </rdfs:subClassOf>
        <rdfs:subClassOf>
            <owl:Restriction>
                <owl:onProperty rdf:resource="&ns4;#sha1checksum"/>
                <owl:maxQualifiedCardinality rdf:datatype="&xsd;nonNegativeInteger">1</owl:maxQualifiedCardinality>
                <owl:onDataRange rdf:resource="&xsd;hexBinary"/>
            </owl:Restriction>
        </rdfs:subClassOf>
        <rdfs:subClassOf>
            <owl:Restriction>
                <owl:onProperty rdf:resource="&ns4;#checksum"/>
                <owl:minQualifiedCardinality rdf:datatype="&xsd;nonNegativeInteger">1</owl:minQualifiedCardinality>
                <owl:onDataRange rdf:resource="&xsd;hexBinary"/>
            </owl:Restriction>
        </rdfs:subClassOf>
        <rdfs:subClassOf>
            <owl:Restriction>
                <owl:onProperty rdf:resource="&ns4;#md5checksum"/>
                <owl:maxQualifiedCardinality rdf:datatype="&xsd;nonNegativeInteger">1</owl:maxQualifiedCardinality>
                <owl:onDataRange rdf:resource="&xsd;hexBinary"/>
            </owl:Restriction>
        </rdfs:subClassOf>
        <rdfs:subClassOf>
            <owl:Restriction>
                <owl:onProperty rdf:resource="&ns4;#compositionLevel"/>
                <owl:maxQualifiedCardinality rdf:datatype="&xsd;nonNegativeInteger">1</owl:maxQualifiedCardinality>
                <owl:onDataRange rdf:resource="&xsd;integer"/>
            </owl:Restriction>
        </rdfs:subClassOf>
        <rdfs:subClassOf>
            <owl:Restriction>
                <owl:onProperty rdf:resource="&ns4;#objectCategory"/>
                <owl:maxQualifiedCardinality rdf:datatype="&xsd;nonNegativeInteger">1</owl:maxQualifiedCardinality>
                <owl:onDataRange rdf:resource="&xsd;string"/>
            </owl:Restriction>
        </rdfs:subClassOf>
        <rdfs:subClassOf>
            <owl:Restriction>
                <owl:onProperty rdf:resource="&ns4;#sha256checksum"/>
                <owl:maxQualifiedCardinality rdf:datatype="&xsd;nonNegativeInteger">1</owl:maxQualifiedCardinality>
                <owl:onDataRange rdf:resource="&xsd;hexBinary"/>
            </owl:Restriction>
        </rdfs:subClassOf>
        <rdfs:subClassOf>
            <owl:Restriction>
                <owl:onProperty rdf:resource="&ns4;#sourceCapture"/>
                <owl:onClass rdf:resource="&ns4;#SourceCapture"/>
                <owl:maxQualifiedCardinality rdf:datatype="&xsd;nonNegativeInteger">1</owl:maxQualifiedCardinality>
            </owl:Restriction>
        </rdfs:subClassOf>
        <rdfs:subClassOf>
            <owl:Restriction>
                <owl:onProperty rdf:resource="&ns4;#size"/>
                <owl:qualifiedCardinality rdf:datatype="&xsd;nonNegativeInteger">1</owl:qualifiedCardinality>
                <owl:onDataRange rdf:resource="&xsd;integer"/>
            </owl:Restriction>
        </rdfs:subClassOf>
        <rdfs:subClassOf>
            <owl:Restriction>
                <owl:onProperty rdf:resource="&ns4;#object"/>
                <owl:onClass rdf:resource="&ns4;#Object"/>
                <owl:qualifiedCardinality rdf:datatype="&xsd;nonNegativeInteger">1</owl:qualifiedCardinality>
            </owl:Restriction>
        </rdfs:subClassOf>
        <rdfs:subClassOf>
            <owl:Restriction>
                <owl:onProperty rdf:resource="&ns4;#formatVersion"/>
                <owl:maxQualifiedCardinality rdf:datatype="&xsd;nonNegativeInteger">1</owl:maxQualifiedCardinality>
                <owl:onDataRange rdf:resource="&xsd;string"/>
            </owl:Restriction>
        </rdfs:subClassOf>
        <rdfs:subClassOf>
            <owl:Restriction>
                <owl:onProperty rdf:resource="&ns4;#sha512checksum"/>
                <owl:maxQualifiedCardinality rdf:datatype="&xsd;nonNegativeInteger">1</owl:maxQualifiedCardinality>
                <owl:onDataRange rdf:resource="&xsd;hexBinary"/>
            </owl:Restriction>
        </rdfs:subClassOf>
        <rdfs:subClassOf>
            <owl:Restriction>
                <owl:onProperty rdf:resource="&ns4;#use"/>
                <owl:qualifiedCardinality rdf:datatype="&xsd;nonNegativeInteger">1</owl:qualifiedCardinality>
                <owl:onDataRange rdf:resource="&xsd;string"/>
            </owl:Restriction>
        </rdfs:subClassOf>
        <rdfs:subClassOf>
            <owl:Restriction>
                <owl:onProperty rdf:resource="&ns4;#dateCreatedByApplication"/>
                <owl:allValuesFrom rdf:resource="&xsd;dateTime"/>
            </owl:Restriction>
        </rdfs:subClassOf>
        <rdfs:subClassOf>
            <owl:Restriction>
                <owl:onProperty rdf:resource="&ns4;#formatName"/>
                <owl:maxQualifiedCardinality rdf:datatype="&xsd;nonNegativeInteger">1</owl:maxQualifiedCardinality>
                <owl:onDataRange rdf:resource="&xsd;string"/>
            </owl:Restriction>
        </rdfs:subClassOf>
        <rdfs:subClassOf>
            <owl:Restriction>
                <owl:onProperty rdf:resource="&ns4;#crc32checksum"/>
                <owl:maxQualifiedCardinality rdf:datatype="&xsd;nonNegativeInteger">1</owl:maxQualifiedCardinality>
                <owl:onDataRange rdf:resource="&xsd;hexBinary"/>
            </owl:Restriction>
        </rdfs:subClassOf>
        <rdfs:comment>Mandatory event: file ingest.</rdfs:comment>
        <rdfs:comment>Must link to the object the file is associated with. If associated with
      a component, must also link to it.</rdfs:comment>
        <rdfs:comment>Ontology: METS</rdfs:comment>
        <rdfs:comment>Mandatory checksum: initial ingest checksum. Currently have best
      coverage in crc32, switch to sha256?</rdfs:comment>
        <rdfs:comment>A file containing content capable of being rendered by a computer.
      May be of any mime type. The DAMS includes a description of each master file,
      that supports its preservation management.</rdfs:comment>
    </owl:Class>
    


    <!-- http://library.ucsd.edu/ontology/dams/#Language -->

    <owl:Class rdf:about="&ns4;#Language">
        <rdfs:label>Language</rdfs:label>
        <rdfs:subClassOf rdf:resource="&ns4;#VocabularyEntry"/>
        <rdfs:comment>The language(s) of the collection, object, or object component
      (ISO 639-2).</rdfs:comment>
    </owl:Class>
    


    <!-- http://library.ucsd.edu/ontology/dams/#License -->

    <owl:Class rdf:about="&ns4;#License">
        <rdfs:label>License</rdfs:label>
        <rdfs:subClassOf rdf:resource="&ns4;#Rights"/>
        <rdfs:subClassOf>
            <owl:Restriction>
                <owl:onProperty rdf:resource="&ns4;#licenseURI"/>
                <owl:allValuesFrom rdf:resource="&xsd;anyURI"/>
            </owl:Restriction>
        </rdfs:subClassOf>
        <rdfs:subClassOf>
            <owl:Restriction>
                <owl:onProperty rdf:resource="&ns4;#licenseNote"/>
                <owl:maxQualifiedCardinality rdf:datatype="&xsd;nonNegativeInteger">1</owl:maxQualifiedCardinality>
                <owl:onDataRange rdf:resource="&xsd;string"/>
            </owl:Restriction>
        </rdfs:subClassOf>
        <rdfs:subClassOf>
            <owl:Restriction>
                <owl:onProperty rdf:resource="&ns4;#rightsAction"/>
                <owl:onClass rdf:resource="&ns4;#RightsAction"/>
                <owl:minQualifiedCardinality rdf:datatype="&xsd;nonNegativeInteger">1</owl:minQualifiedCardinality>
            </owl:Restriction>
        </rdfs:subClassOf>
        <rdfs:subClassOf>
            <owl:Restriction>
                <owl:onProperty rdf:resource="&ns4;#relationship"/>
                <owl:onClass rdf:resource="&ns4;#Relationship"/>
                <owl:minQualifiedCardinality rdf:datatype="&xsd;nonNegativeInteger">1</owl:minQualifiedCardinality>
            </owl:Restriction>
        </rdfs:subClassOf>
        <rdfs:comment>Licenses statements must link to permission and/or restrictions statements, and
      those statements link to dates. Thus, license statements do not directly link to dates. The
      active dates of the license should be capable of being inferred from the whole of the related
      permission / restriction statements, if there is cause to assign a collective date to a
      license.</rdfs:comment>
        <rdfs:comment>A contract between the rights holder for content and the repository indicating
      the rights and constraints placed upon the content for the repository. Purchase agreements,
      deeds of gift, transfer agreements are construable as kinds of licenses.</rdfs:comment>
        <rdfs:comment>Required name/role: rights holder.</rdfs:comment>
        <rdfs:comment>It is possible for a license to be granted at specific time but for some or
      all eventual permissions to be restricted for a period of time initially. This is basically
      how embargoed ETDs are now modeled in the DAMS.</rdfs:comment>
    </owl:Class>
    


    <!-- http://library.ucsd.edu/ontology/dams/#Name -->

    <owl:Class rdf:about="&ns4;#Name">
        <rdfs:subClassOf rdf:resource="&ns4;#VocabularyEntry"/>
        <rdfs:subClassOf>
            <owl:Restriction>
                <owl:onProperty rdf:resource="&ns4;#type"/>
                <owl:qualifiedCardinality rdf:datatype="&xsd;nonNegativeInteger">1</owl:qualifiedCardinality>
                <owl:onDataRange>
                    <rdfs:Datatype>
                        <owl:oneOf>
                            <rdf:Description>
                                <rdf:type rdf:resource="&rdf;List"/>
                                <rdf:first rdf:datatype="&xsd;string">&#39;personal&#39;, &#39;corporate&#39;, &#39;conference&#39;, &#39;family&#39;, &#39;software&#39;</rdf:first>
                                <rdf:rest rdf:resource="&rdf;nil"/>
                            </rdf:Description>
                        </owl:oneOf>
                    </rdfs:Datatype>
                </owl:onDataRange>
            </owl:Restriction>
        </rdfs:subClassOf>
        <rdfs:subClassOf>
            <owl:Restriction>
                <owl:onProperty rdf:resource="&ns4;#authority"/>
                <owl:allValuesFrom>
                    <rdfs:Datatype>
                        <owl:oneOf>
                            <rdf:Description>
                                <rdf:type rdf:resource="&rdf;List"/>
                                <rdf:first rdf:datatype="&xsd;string">&#39;abne&#39;, &#39;bibalex&#39;, &#39;conorsi&#39;, &#39;gkd&#39;, &#39;gnd&#39;, &#39;hapi&#39;, &#39;hkcan&#39;, &#39;lacnaf&#39;, &#39;naf&#39;, &#39;nalnaf&#39;, &#39;nlmnaf&#39;, &#39;nznb&#39;, &#39;sanb&#39;, &#39;ulan&#39;, &#39;unbisn&#39;</rdf:first>
                                <rdf:rest rdf:resource="&rdf;nil"/>
                            </rdf:Description>
                        </owl:oneOf>
                    </rdfs:Datatype>
                </owl:allValuesFrom>
            </owl:Restriction>
        </rdfs:subClassOf>
        <rdfs:comment>The name may be composed of name parts per its type as a personal,
      family, or corporate body name.  (See http://www.loc.gov/standards/mods/userguide/name.html</rdfs:comment>
        <rdfs:comment>The name form for a person, family, corporate body, or software
      agent represented in the DAMS and pertinent to a collection, object, object
      component, rights statement, or event.</rdfs:comment>
        <rdfs:comment>Display form to be generated from name parts by presentation process</rdfs:comment>
        <rdfs:comment>DisplayLabel should be suppressed.</rdfs:comment>
    </owl:Class>
    


    <!-- http://library.ucsd.edu/ontology/dams/#Note -->

    <owl:Class rdf:about="&ns4;#Note">
        <rdfs:label>Note</rdfs:label>
        <rdfs:subClassOf rdf:resource="&ns4;#DAMSThing"/>
        <rdfs:subClassOf>
            <owl:Restriction>
                <owl:onProperty rdf:resource="&ns4;#value"/>
                <owl:qualifiedCardinality rdf:datatype="&xsd;nonNegativeInteger">1</owl:qualifiedCardinality>
                <owl:onDataRange rdf:resource="&xsd;string"/>
            </owl:Restriction>
        </rdfs:subClassOf>
        <rdfs:subClassOf>
            <owl:Restriction>
                <owl:onProperty rdf:resource="&ns4;#displayLabel"/>
                <owl:maxQualifiedCardinality rdf:datatype="&xsd;nonNegativeInteger">1</owl:maxQualifiedCardinality>
                <owl:onDataRange rdf:resource="&xsd;string"/>
            </owl:Restriction>
        </rdfs:subClassOf>
        <rdfs:subClassOf>
            <owl:Restriction>
                <owl:onProperty rdf:resource="&ns4;#type"/>
                <owl:allValuesFrom>
                    <rdfs:Datatype>
                        <owl:oneOf>
                            <rdf:Description>
                                <rdf:type rdf:resource="&rdf;List"/>
                                <rdf:first rdf:datatype="&xsd;string">&#39;abstract&#39;, &#39;inscription&#39;, &#39;identifier:doi&#39;, &#39;identifier:filename&#39;, &#39;identifier:local&#39;, &#39;extent&#39;, &#39;digitalOrigin&#39;</rdf:first>
                                <rdf:rest rdf:resource="&rdf;nil"/>
                            </rdf:Description>
                        </owl:oneOf>
                    </rdfs:Datatype>
                </owl:allValuesFrom>
            </owl:Restriction>
        </rdfs:subClassOf>
        <rdfs:subClassOf>
            <owl:Restriction>
                <owl:onProperty rdf:resource="&ns4;#internalOnly"/>
                <owl:qualifiedCardinality rdf:datatype="&xsd;nonNegativeInteger">1</owl:qualifiedCardinality>
                <owl:onDataRange rdf:resource="&xsd;boolean"/>
            </owl:Restriction>
        </rdfs:subClassOf>
        <rdfs:comment>A description of some facet of a collection, object, or object component. Facets
      may range form abstract and scope content notes to specific aspects such as rights
      status.</rdfs:comment>
        <rdfs:comment>mods:originInfo will be created as an unstructured note.</rdfs:comment>
    </owl:Class>
    


    <!-- http://library.ucsd.edu/ontology/dams/#Object -->

    <owl:Class rdf:about="&ns4;#Object">
        <rdfs:label>Object</rdfs:label>
        <rdfs:subClassOf rdf:resource="&ns4;#DAMSResource"/>
        <rdfs:subClassOf>
            <owl:Restriction>
                <owl:onProperty rdf:resource="&ns4;#language"/>
                <owl:onClass rdf:resource="&ns4;#Language"/>
                <owl:minQualifiedCardinality rdf:datatype="&xsd;nonNegativeInteger">1</owl:minQualifiedCardinality>
            </owl:Restriction>
        </rdfs:subClassOf>
        <rdfs:subClassOf>
            <owl:Restriction>
                <owl:onProperty rdf:resource="&ns4;#license"/>
                <owl:onClass rdf:resource="&ns4;#License"/>
                <owl:maxQualifiedCardinality rdf:datatype="&xsd;nonNegativeInteger">1</owl:maxQualifiedCardinality>
            </owl:Restriction>
        </rdfs:subClassOf>
        <rdfs:subClassOf>
            <owl:Restriction>
                <owl:onProperty rdf:resource="&ns4;#copyright"/>
                <owl:onClass rdf:resource="&ns4;#Copyright"/>
                <owl:qualifiedCardinality rdf:datatype="&xsd;nonNegativeInteger">1</owl:qualifiedCardinality>
            </owl:Restriction>
        </rdfs:subClassOf>
        <rdfs:subClassOf>
            <owl:Restriction>
                <owl:onProperty rdf:resource="&ns4;#otherRights"/>
                <owl:onClass rdf:resource="&ns4;#OtherRights"/>
                <owl:maxQualifiedCardinality rdf:datatype="&xsd;nonNegativeInteger">1</owl:maxQualifiedCardinality>
            </owl:Restriction>
        </rdfs:subClassOf>
        <rdfs:subClassOf>
            <owl:Restriction>
                <owl:onProperty rdf:resource="&ns4;#statute"/>
                <owl:onClass rdf:resource="&ns4;#Statute"/>
                <owl:maxQualifiedCardinality rdf:datatype="&xsd;nonNegativeInteger">1</owl:maxQualifiedCardinality>
            </owl:Restriction>
        </rdfs:subClassOf>
        <rdfs:subClassOf>
            <owl:Restriction>
                <owl:onProperty rdf:resource="&ns4;#title"/>
                <owl:onClass rdf:resource="&ns4;#Title"/>
                <owl:minQualifiedCardinality rdf:datatype="&xsd;nonNegativeInteger">1</owl:minQualifiedCardinality>
            </owl:Restriction>
        </rdfs:subClassOf>
        <rdfs:subClassOf>
            <owl:Restriction>
                <owl:onProperty rdf:resource="&ns4;#repository"/>
                <owl:onClass rdf:resource="&ns4;#Repository"/>
                <owl:qualifiedCardinality rdf:datatype="&xsd;nonNegativeInteger">1</owl:qualifiedCardinality>
            </owl:Restriction>
        </rdfs:subClassOf>
        <rdfs:comment>A representation of an intellectual entity, sometimes referred
      to as a &quot;work.&quot; The object is composed of three distinct types of
      information: 1) one or more content files, 2) one or more metadata records,
      and 3) a binder (unique ID) holding all the parts of the object together and
      maintaining the correct internal associations among the parts.</rdfs:comment>
        <rdfs:comment>Every object must be linked to one, and only one, Repository.
      It may be linked to as many collections as are pertinent.</rdfs:comment>
        <rdfs:comment>Title and Language: cardinality overrides superclass.</rdfs:comment>
        <rdfs:comment>Mandatory event: object creation.</rdfs:comment>
        <rdfs:comment>DAMS Object requirements need to be changed to reflect this
      (RCI Levy &amp; SIO examples)</rdfs:comment>
    </owl:Class>
    


    <!-- http://library.ucsd.edu/ontology/dams/#OtherRights -->

    <owl:Class rdf:about="&ns4;#OtherRights">
        <rdfs:subClassOf rdf:resource="&ns4;#Rights"/>
        <rdfs:subClassOf>
            <owl:Restriction>
                <owl:onProperty rdf:resource="&ns4;#rightsAction"/>
                <owl:onClass rdf:resource="&ns4;#RightsAction"/>
                <owl:minQualifiedCardinality rdf:datatype="&xsd;nonNegativeInteger">1</owl:minQualifiedCardinality>
            </owl:Restriction>
        </rdfs:subClassOf>
        <rdfs:subClassOf>
            <owl:Restriction>
                <owl:onProperty rdf:resource="&ns4;#otherRightsURI"/>
                <owl:maxQualifiedCardinality rdf:datatype="&xsd;nonNegativeInteger">1</owl:maxQualifiedCardinality>
                <owl:onDataRange rdf:resource="&xsd;anyURI"/>
            </owl:Restriction>
        </rdfs:subClassOf>
        <rdfs:subClassOf>
            <owl:Restriction>
                <owl:onProperty rdf:resource="&ns4;#relationship"/>
                <owl:onClass rdf:resource="&ns4;#Relationship"/>
                <owl:qualifiedCardinality rdf:datatype="&xsd;nonNegativeInteger">1</owl:qualifiedCardinality>
            </owl:Restriction>
        </rdfs:subClassOf>
        <rdfs:subClassOf>
            <owl:Restriction>
                <owl:onProperty rdf:resource="&ns4;#otherRightsBasis"/>
                <owl:qualifiedCardinality rdf:datatype="&xsd;nonNegativeInteger">1</owl:qualifiedCardinality>
                <owl:onDataRange rdf:resource="&xsd;string"/>
            </owl:Restriction>
        </rdfs:subClassOf>
        <rdfs:subClassOf>
            <owl:Restriction>
                <owl:onProperty rdf:resource="&ns4;#otherRightsNote"/>
                <owl:maxQualifiedCardinality rdf:datatype="&xsd;nonNegativeInteger">1</owl:maxQualifiedCardinality>
                <owl:onDataRange rdf:resource="&xsd;string"/>
            </owl:Restriction>
        </rdfs:subClassOf>
        <rdfs:comment>Required Relationship: decision maker.</rdfs:comment>
        <rdfs:comment>Any other rights not covered by copyright, statute, or license. This typically
       includes library policies that restrict access to content out of respect to cultural
       sensitivities.</rdfs:comment>
        <rdfs:comment>We currently do not use Other Rights in the DAMS, but that is because this
       element was only recently added to PREMIS. We do have objects that have been restricted
       due to institutional policy, the culturally sensitive objects in Lambert being a case in
       point. We also have objects that UCSD has decided to display under the principles of fair
       use.</rdfs:comment>
        <rdfs:comment>Other Rights, like other right types, link indirectly to dates via Rights Action.</rdfs:comment>
    </owl:Class>
    


    <!-- http://library.ucsd.edu/ontology/dams/#Permission -->

    <owl:Class rdf:about="&ns4;#Permission">
        <rdfs:subClassOf rdf:resource="&ns4;#RightsAction"/>
        <rdfs:comment>An action that is allowed.</rdfs:comment>
    </owl:Class>
    


    <!-- http://library.ucsd.edu/ontology/dams/#PreferredCitationNote -->

    <owl:Class rdf:about="&ns4;#PreferredCitationNote">
        <rdfs:subClassOf rdf:resource="&ns4;#Note"/>
        <rdfs:subClassOf>
            <owl:Restriction>
                <owl:onProperty rdf:resource="&ns4;#type"/>
                <owl:cardinality rdf:datatype="&xsd;nonNegativeInteger">0</owl:cardinality>
            </owl:Restriction>
        </rdfs:subClassOf>
        <rdfs:comment>Investigate automating this value.</rdfs:comment>
        <rdfs:comment>Note containing the preferred citation form.</rdfs:comment>
    </owl:Class>
    


    <!-- http://library.ucsd.edu/ontology/dams/#RelatedResource -->

    <owl:Class rdf:about="&ns4;#RelatedResource">
        <rdfs:subClassOf rdf:resource="&ns4;#DAMSThing"/>
        <rdfs:subClassOf>
            <owl:Restriction>
                <owl:onProperty rdf:resource="&ns4;#type"/>
                <owl:allValuesFrom>
                    <rdfs:Datatype>
                        <owl:oneOf>
                            <rdf:Description>
                                <rdf:type rdf:resource="&rdf;List"/>
                                <rdf:first rdf:datatype="&xsd;string">&#39;online exhibit&#39;, &#39;source&#39;, &#39;parallel description&#39;, &#39;depicts&#39;, &#39;derived from&#39;</rdf:first>
                                <rdf:rest rdf:resource="&rdf;nil"/>
                            </rdf:Description>
                        </owl:oneOf>
                    </rdfs:Datatype>
                </owl:allValuesFrom>
            </owl:Restriction>
        </rdfs:subClassOf>
        <rdfs:subClassOf>
            <owl:Restriction>
                <owl:onProperty rdf:resource="&ns4;#description"/>
                <owl:maxQualifiedCardinality rdf:datatype="&xsd;nonNegativeInteger">1</owl:maxQualifiedCardinality>
                <owl:onDataRange rdf:resource="&xsd;string"/>
            </owl:Restriction>
        </rdfs:subClassOf>
        <rdfs:subClassOf>
            <owl:Restriction>
                <owl:onProperty rdf:resource="&ns4;#uri"/>
                <owl:allValuesFrom rdf:resource="&xsd;anyURI"/>
            </owl:Restriction>
        </rdfs:subClassOf>
        <rdfs:comment>We may need to either write policy to enforce relationships between classes
      (object to object, collection to collection, etc.) or subclass Related Resource to enforce
      relationships.</rdfs:comment>
        <rdfs:comment>Describes a related resource either internal to the DAMS or in a system external
      to the DAMS. This could include metadata in another format, content version in another
      system, relationship between objects and relationship between collections in respect to
      a specified property.</rdfs:comment>
    </owl:Class>
    


    <!-- http://library.ucsd.edu/ontology/dams/#Relationship -->

    <owl:Class rdf:about="&ns4;#Relationship">
        <rdfs:label>Relationship</rdfs:label>
        <rdfs:subClassOf rdf:resource="&ns4;#DAMSThing"/>
        <rdfs:subClassOf>
            <owl:Restriction>
                <owl:onProperty rdf:resource="&ns4;#name"/>
                <owl:onClass rdf:resource="&ns4;#Name"/>
                <owl:qualifiedCardinality rdf:datatype="&xsd;nonNegativeInteger">1</owl:qualifiedCardinality>
            </owl:Restriction>
        </rdfs:subClassOf>
        <rdfs:subClassOf>
            <owl:Restriction>
                <owl:onProperty rdf:resource="&ns4;#role"/>
                <owl:onClass rdf:resource="&ns4;#Role"/>
                <owl:minQualifiedCardinality rdf:datatype="&xsd;nonNegativeInteger">1</owl:minQualifiedCardinality>
            </owl:Restriction>
        </rdfs:subClassOf>
        <rdfs:comment>Name/Role bundle which is linked to from Collection, Object, etc.</rdfs:comment>
    </owl:Class>
    


    <!-- http://library.ucsd.edu/ontology/dams/#Repository -->

    <owl:Class rdf:about="&ns4;#Repository">
        <rdfs:label>Repository</rdfs:label>
        <rdfs:subClassOf rdf:resource="&ns4;#DAMSThing"/>
        <rdfs:subClassOf>
            <owl:Restriction>
                <owl:onProperty rdf:resource="&ns4;#event"/>
                <owl:onClass rdf:resource="&ns4;#DAMSEvent"/>
                <owl:minQualifiedCardinality rdf:datatype="&xsd;nonNegativeInteger">1</owl:minQualifiedCardinality>
            </owl:Restriction>
        </rdfs:subClassOf>
        <rdfs:subClassOf>
            <owl:Restriction>
                <owl:onProperty rdf:resource="&ns4;#repositoryURI"/>
                <owl:maxQualifiedCardinality rdf:datatype="&xsd;nonNegativeInteger">1</owl:maxQualifiedCardinality>
                <owl:onDataRange rdf:resource="&xsd;anyURI"/>
            </owl:Restriction>
        </rdfs:subClassOf>
        <rdfs:subClassOf>
            <owl:Restriction>
                <owl:onProperty rdf:resource="&ns4;#repositoryName"/>
                <owl:qualifiedCardinality rdf:datatype="&xsd;nonNegativeInteger">1</owl:qualifiedCardinality>
                <owl:onDataRange rdf:resource="&xsd;string"/>
            </owl:Restriction>
        </rdfs:subClassOf>
        <rdfs:comment>The identification of a library unit (or non-library data provider)
      that is responsible for supplying content to the DAMS and for administering that
      content over time, including answering queries from users.</rdfs:comment>
        <rdfs:comment>All objects in the DAMS must be linked to one and only one repository.</rdfs:comment>
        <rdfs:comment>Mandatory event: repository record creation.</rdfs:comment>
        <rdfs:comment>Will revisit the need for Agency Code and Country Code properties. These
      attributes may be conducive for sharing records.</rdfs:comment>
    </owl:Class>
    


    <!-- http://library.ucsd.edu/ontology/dams/#Restriction -->

    <owl:Class rdf:about="&ns4;#Restriction">
        <rdfs:subClassOf rdf:resource="&ns4;#RightsAction"/>
        <rdfs:subClassOf>
            <owl:Restriction>
                <owl:onProperty rdf:resource="&ns4;#endDate"/>
                <owl:qualifiedCardinality rdf:datatype="&xsd;nonNegativeInteger">1</owl:qualifiedCardinality>
                <owl:onDataRange rdf:resource="&xsd;date"/>
            </owl:Restriction>
        </rdfs:subClassOf>
        <rdfs:comment>An action is not allowed.</rdfs:comment>
    </owl:Class>
    


    <!-- http://library.ucsd.edu/ontology/dams/#Rights -->

    <owl:Class rdf:about="&ns4;#Rights">
        <rdfs:subClassOf rdf:resource="&ns4;#DAMSThing"/>
        <rdfs:subClassOf>
            <owl:Restriction>
                <owl:onProperty rdf:resource="&ns4;#event"/>
                <owl:allValuesFrom rdf:resource="&ns4;#DAMSEvent"/>
            </owl:Restriction>
        </rdfs:subClassOf>
        <rdfs:comment>Superclass of classes which describe intellectual property rights which allow
      or deny access to an item.</rdfs:comment>
    </owl:Class>
    


    <!-- http://library.ucsd.edu/ontology/dams/#RightsAction -->

    <owl:Class rdf:about="&ns4;#RightsAction">
        <rdfs:subClassOf rdf:resource="&ns4;#DAMSThing"/>
        <rdfs:subClassOf>
            <owl:Restriction>
                <owl:onProperty rdf:resource="&ns4;#endDate"/>
                <owl:allValuesFrom rdf:resource="&xsd;date"/>
            </owl:Restriction>
        </rdfs:subClassOf>
        <rdfs:subClassOf>
            <owl:Restriction>
                <owl:onProperty rdf:resource="&ns4;#type"/>
                <owl:qualifiedCardinality rdf:datatype="&xsd;nonNegativeInteger">1</owl:qualifiedCardinality>
                <owl:onDataRange>
                    <rdfs:Datatype>
                        <owl:oneOf>
                            <rdf:Description>
                                <rdf:type rdf:resource="&rdf;List"/>
                                <rdf:first rdf:datatype="&xsd;string">&#39;display&#39;, &#39;migrate&#39;, &#39;replicate&#39;, &#39;modify&#39;</rdf:first>
                                <rdf:rest rdf:resource="&rdf;nil"/>
                            </rdf:Description>
                        </owl:oneOf>
                    </rdfs:Datatype>
                </owl:onDataRange>
            </owl:Restriction>
        </rdfs:subClassOf>
        <rdfs:subClassOf>
            <owl:Restriction>
                <owl:onProperty rdf:resource="&ns4;#beginDate"/>
                <owl:allValuesFrom rdf:resource="&xsd;date"/>
            </owl:Restriction>
        </rdfs:subClassOf>
        <rdfs:comment>An action that is permitted or restricted according to the rights status for an
       object or object component.</rdfs:comment>
    </owl:Class>
    


    <!-- http://library.ucsd.edu/ontology/dams/#Role -->

    <owl:Class rdf:about="&ns4;#Role">
        <rdfs:label>Role</rdfs:label>
        <rdfs:subClassOf rdf:resource="&ns4;#VocabularyEntry"/>
        <rdfs:subClassOf>
            <owl:Restriction>
                <owl:onProperty rdf:resource="&ns4;#term"/>
                <owl:allValuesFrom>
                    <rdfs:Datatype>
                        <owl:oneOf>
                            <rdf:Description>
                                <rdf:type rdf:resource="&rdf;List"/>
                                <rdf:first rdf:datatype="&xsd;string">&#39;creator&#39;, &#39;author&#39;, &#39;publisher&#39;</rdf:first>
                                <rdf:rest rdf:resource="&rdf;nil"/>
                            </rdf:Description>
                        </owl:oneOf>
                    </rdfs:Datatype>
                </owl:allValuesFrom>
            </owl:Restriction>
        </rdfs:subClassOf>
        <rdfs:comment>A term describing the relationship between a Name and an Collection, Object,
      Component, Events, and Rights Status.</rdfs:comment>
        <rdfs:comment>A list of terms for the relationship of name to Collection, Object, Component,
      Events, and Rights Status. The predicates can be derived from standard and local list of
      role terms. Role may be a subclass of higher level entity such as Functional
      Relationship.</rdfs:comment>
    </owl:Class>
    


    <!-- http://library.ucsd.edu/ontology/dams/#ScopeContentNote -->

    <owl:Class rdf:about="&ns4;#ScopeContentNote">
        <rdfs:subClassOf rdf:resource="&ns4;#Note"/>
        <rdfs:subClassOf>
            <owl:Restriction>
                <owl:onProperty rdf:resource="&ns4;#type"/>
                <owl:cardinality rdf:datatype="&xsd;nonNegativeInteger">0</owl:cardinality>
            </owl:Restriction>
        </rdfs:subClassOf>
        <rdfs:comment>Note describing the contents of a collection.</rdfs:comment>
    </owl:Class>
    


    <!-- http://library.ucsd.edu/ontology/dams/#SourceCapture -->

    <owl:Class rdf:about="&ns4;#SourceCapture">
        <rdfs:subClassOf rdf:resource="&ns4;#DAMSThing"/>
        <rdfs:subClassOf>
            <owl:Restriction>
                <owl:onProperty rdf:resource="&ns4;#sourceType"/>
                <owl:maxQualifiedCardinality rdf:datatype="&xsd;nonNegativeInteger">1</owl:maxQualifiedCardinality>
                <owl:onDataRange rdf:resource="&xsd;string"/>
            </owl:Restriction>
        </rdfs:subClassOf>
        <rdfs:subClassOf>
            <owl:Restriction>
                <owl:onProperty rdf:resource="&ns4;#scanningSoftwareVersion"/>
                <owl:maxQualifiedCardinality rdf:datatype="&xsd;nonNegativeInteger">1</owl:maxQualifiedCardinality>
                <owl:onDataRange rdf:resource="&xsd;string"/>
            </owl:Restriction>
        </rdfs:subClassOf>
        <rdfs:subClassOf>
            <owl:Restriction>
                <owl:onProperty rdf:resource="&ns4;#captureSource"/>
                <owl:maxQualifiedCardinality rdf:datatype="&xsd;nonNegativeInteger">1</owl:maxQualifiedCardinality>
                <owl:onDataRange rdf:resource="&xsd;string"/>
            </owl:Restriction>
        </rdfs:subClassOf>
        <rdfs:subClassOf>
            <owl:Restriction>
                <owl:onProperty rdf:resource="&ns4;#scannerManufacturer"/>
                <owl:maxQualifiedCardinality rdf:datatype="&xsd;nonNegativeInteger">1</owl:maxQualifiedCardinality>
                <owl:onDataRange rdf:resource="&xsd;string"/>
            </owl:Restriction>
        </rdfs:subClassOf>
        <rdfs:subClassOf>
            <owl:Restriction>
                <owl:onProperty rdf:resource="&ns4;#scannerModelName"/>
                <owl:maxQualifiedCardinality rdf:datatype="&xsd;nonNegativeInteger">1</owl:maxQualifiedCardinality>
                <owl:onDataRange rdf:resource="&xsd;string"/>
            </owl:Restriction>
        </rdfs:subClassOf>
        <rdfs:subClassOf>
            <owl:Restriction>
                <owl:onProperty rdf:resource="&ns4;#scanningSoftware"/>
                <owl:maxQualifiedCardinality rdf:datatype="&xsd;nonNegativeInteger">1</owl:maxQualifiedCardinality>
                <owl:onDataRange rdf:resource="&xsd;string"/>
            </owl:Restriction>
        </rdfs:subClassOf>
        <rdfs:subClassOf>
            <owl:Restriction>
                <owl:onProperty rdf:resource="&ns4;#imageProducer"/>
                <owl:maxQualifiedCardinality rdf:datatype="&xsd;nonNegativeInteger">1</owl:maxQualifiedCardinality>
                <owl:onDataRange rdf:resource="&xsd;string"/>
            </owl:Restriction>
        </rdfs:subClassOf>
        <rdfs:comment>Ontology: MIX</rdfs:comment>
        <rdfs:comment>An indication of software and hardware used to produce the content file.</rdfs:comment>
    </owl:Class>
    


    <!-- http://library.ucsd.edu/ontology/dams/#Statute -->

    <owl:Class rdf:about="&ns4;#Statute">
        <rdfs:label>Statute</rdfs:label>
        <rdfs:subClassOf rdf:resource="&ns4;#Rights"/>
        <rdfs:subClassOf>
            <owl:Restriction>
                <owl:onProperty rdf:resource="&ns4;#statuteJurisdiction"/>
                <owl:qualifiedCardinality rdf:datatype="&xsd;nonNegativeInteger">1</owl:qualifiedCardinality>
                <owl:onDataRange rdf:resource="&xsd;string"/>
            </owl:Restriction>
        </rdfs:subClassOf>
        <rdfs:subClassOf>
            <owl:Restriction>
                <owl:onProperty rdf:resource="&ns4;#statuteNote"/>
                <owl:maxQualifiedCardinality rdf:datatype="&xsd;nonNegativeInteger">1</owl:maxQualifiedCardinality>
                <owl:onDataRange rdf:resource="&xsd;string"/>
            </owl:Restriction>
        </rdfs:subClassOf>
        <rdfs:subClassOf>
            <owl:Restriction>
                <owl:onProperty rdf:resource="&ns4;#statuteCitation"/>
                <owl:qualifiedCardinality rdf:datatype="&xsd;nonNegativeInteger">1</owl:qualifiedCardinality>
                <owl:onDataRange rdf:resource="&xsd;string"/>
            </owl:Restriction>
        </rdfs:subClassOf>
        <rdfs:subClassOf>
            <owl:Restriction>
                <owl:onProperty rdf:resource="&ns4;#rightsAction"/>
                <owl:onClass rdf:resource="&ns4;#RightsAction"/>
                <owl:minQualifiedCardinality rdf:datatype="&xsd;nonNegativeInteger">1</owl:minQualifiedCardinality>
            </owl:Restriction>
        </rdfs:subClassOf>
        <rdfs:comment>Statutes typically limit access to content in some way, often because the
      content is of a type protected by privacy / confidentiality laws, e.g. FERPA, HIPA,
      etc.</rdfs:comment>
        <rdfs:comment>Currently we do not include in the DAMS any content subject to statutory
      regulation. That, of course, can change.</rdfs:comment>
        <rdfs:comment>Statues link to a permissions and / or restriction records, and they link to
      dates. Thus, statutes link indirectly to dates.</rdfs:comment>
        <rdfs:comment>Required Rights Action: whether the statute allows or prohibits
      display.</rdfs:comment>
        <rdfs:comment>A national or regional statute that pertains to content and typically limits
      access to it on some degree, e.g. Federal Educational Rights and Privacy Act (FERPA), which
      limits dissemination of student records for a specified period of time.</rdfs:comment>
    </owl:Class>
    


    <!-- http://library.ucsd.edu/ontology/dams/#Subject -->

    <owl:Class rdf:about="&ns4;#Subject">
        <rdfs:label>Subject</rdfs:label>
        <rdfs:subClassOf rdf:resource="&ns4;#VocabularyEntry"/>
        <rdfs:subClassOf>
            <owl:Restriction>
                <owl:onProperty rdf:resource="&ns4;#authority"/>
                <owl:allValuesFrom>
                    <rdfs:Datatype>
                        <owl:oneOf>
                            <rdf:Description>
                                <rdf:type rdf:resource="&rdf;List"/>
                                <rdf:first rdf:datatype="&xsd;string">&#39;aat&#39;, &#39;naf&#39;, &#39;lcsh&#39;, &#39;mesh&#39;, &#39;tgn&#39;, &#39;local&#39;</rdf:first>
                                <rdf:rest rdf:resource="&rdf;nil"/>
                            </rdf:Description>
                        </owl:oneOf>
                    </rdfs:Datatype>
                </owl:allValuesFrom>
            </owl:Restriction>
        </rdfs:subClassOf>
        <rdfs:subClassOf>
            <owl:Restriction>
                <owl:onProperty rdf:resource="&ns4;#cartographics"/>
                <owl:onClass rdf:resource="&ns4;#Cartographics"/>
                <owl:maxQualifiedCardinality rdf:datatype="&xsd;nonNegativeInteger">1</owl:maxQualifiedCardinality>
            </owl:Restriction>
        </rdfs:subClassOf>
        <rdfs:subClassOf>
            <owl:Restriction>
                <owl:onProperty rdf:resource="&ns4;#title"/>
                <owl:onClass rdf:resource="&ns4;#Title"/>
                <owl:maxQualifiedCardinality rdf:datatype="&xsd;nonNegativeInteger">1</owl:maxQualifiedCardinality>
            </owl:Restriction>
        </rdfs:subClassOf>
        <rdfs:subClassOf>
            <owl:Restriction>
                <owl:onProperty rdf:resource="&ns4;#name"/>
                <owl:onClass rdf:resource="&ns4;#Name"/>
                <owl:maxQualifiedCardinality rdf:datatype="&xsd;nonNegativeInteger">1</owl:maxQualifiedCardinality>
            </owl:Restriction>
        </rdfs:subClassOf>
        <rdfs:subClassOf>
            <owl:Restriction>
                <owl:onProperty rdf:resource="&ns4;#subjectPart"/>
                <owl:allValuesFrom rdf:resource="&ns4;#SubjectPart"/>
            </owl:Restriction>
        </rdfs:subClassOf>
        <rdfs:comment>term and displayLabel should be suppressed.</rdfs:comment>
        <rdfs:comment>Additional rules TBD.</rdfs:comment>
        <rdfs:comment>Look at MADS class &quot;authority&quot; (and subclasses) for modeling of subject
      and possibly name.</rdfs:comment>
        <rdfs:comment>Subject headings may include subject parts.</rdfs:comment>
        <rdfs:comment>A heading indicating the content of the collection, object, or object component.
      Subject headings may be specified as topic, genre/form, geographical name, title, function,
      occupation, title, name, cartographics, etc.</rdfs:comment>
        <rdfs:comment>Subject requires one of: Title, Name, Subject Part, Cartographics</rdfs:comment>
    </owl:Class>
    


    <!-- http://library.ucsd.edu/ontology/dams/#SubjectPart -->

    <owl:Class rdf:about="&ns4;#SubjectPart">
        <rdfs:subClassOf rdf:resource="&ns4;#VocabularyEntry"/>
        <rdfs:subClassOf>
            <owl:Restriction>
                <owl:onProperty rdf:resource="&ns4;#type"/>
                <owl:qualifiedCardinality rdf:datatype="&xsd;nonNegativeInteger">1</owl:qualifiedCardinality>
                <owl:onDataRange>
                    <rdfs:Datatype>
                        <owl:oneOf>
                            <rdf:Description>
                                <rdf:type rdf:resource="&rdf;List"/>
                                <rdf:first rdf:datatype="&xsd;string">&#39;topic&#39;, &#39;geographic&#39;, &#39;temporal&#39;, &#39;genre&#39;, &#39;occupation&#39;,&#39;function&#39;,&#39;culturalContext&#39;,&#39;stylePeriod&#39;,&#39;scientificName&#39;,&#39;buildworkPlace&#39;,&#39;iconography&#39;,&#39;technique&#39;</rdf:first>
                                <rdf:rest rdf:resource="&rdf;nil"/>
                            </rdf:Description>
                        </owl:oneOf>
                    </rdfs:Datatype>
                </owl:onDataRange>
            </owl:Restriction>
        </rdfs:subClassOf>
        <rdfs:subClassOf>
            <owl:Restriction>
                <owl:onProperty rdf:resource="&ns4;#order"/>
                <owl:cardinality rdf:datatype="&xsd;nonNegativeInteger">1</owl:cardinality>
            </owl:Restriction>
        </rdfs:subClassOf>
        <rdfs:comment>A singular subject term, which may be added to other subject terms to compose
      a complete subject expression for a collection, object, or object component.</rdfs:comment>
    </owl:Class>
    


    <!-- http://library.ucsd.edu/ontology/dams/#Title -->

    <owl:Class rdf:about="&ns4;#Title">
        <rdfs:label>Title</rdfs:label>
        <rdfs:subClassOf rdf:resource="&ns4;#DAMSThing"/>
        <rdfs:subClassOf>
            <owl:Restriction>
                <owl:onProperty rdf:resource="&ns4;#authority"/>
                <owl:maxQualifiedCardinality rdf:datatype="&xsd;nonNegativeInteger">1</owl:maxQualifiedCardinality>
                <owl:onDataRange rdf:resource="&xsd;string"/>
            </owl:Restriction>
        </rdfs:subClassOf>
        <rdfs:subClassOf>
            <owl:Restriction>
                <owl:onProperty rdf:resource="&ns4;#partName"/>
                <owl:maxQualifiedCardinality rdf:datatype="&xsd;nonNegativeInteger">1</owl:maxQualifiedCardinality>
                <owl:onDataRange rdf:resource="&xsd;string"/>
            </owl:Restriction>
        </rdfs:subClassOf>
        <rdfs:subClassOf>
            <owl:Restriction>
                <owl:onProperty rdf:resource="&ns4;#value"/>
                <owl:qualifiedCardinality rdf:datatype="&xsd;nonNegativeInteger">1</owl:qualifiedCardinality>
                <owl:onDataRange rdf:resource="&xsd;string"/>
            </owl:Restriction>
        </rdfs:subClassOf>
        <rdfs:subClassOf>
            <owl:Restriction>
                <owl:onProperty rdf:resource="&ns4;#type"/>
                <owl:allValuesFrom>
                    <rdfs:Datatype>
                        <owl:oneOf>
                            <rdf:Description>
                                <rdf:type rdf:resource="&rdf;List"/>
                                <rdf:first rdf:datatype="&xsd;string">&#39;translated&#39;, &#39;transliterated&#39;, &#39;enumerated&#39;, &#39;abbreviated&#39;, &#39;uniform&#39;, &#39;main&#39;, &#39;alternative&#39;</rdf:first>
                                <rdf:rest rdf:resource="&rdf;nil"/>
                            </rdf:Description>
                        </owl:oneOf>
                    </rdfs:Datatype>
                </owl:allValuesFrom>
            </owl:Restriction>
        </rdfs:subClassOf>
        <rdfs:subClassOf>
            <owl:Restriction>
                <owl:onProperty rdf:resource="&ns4;#nonsortCharacters"/>
                <owl:maxQualifiedCardinality rdf:datatype="&xsd;nonNegativeInteger">1</owl:maxQualifiedCardinality>
                <owl:onDataRange rdf:resource="&xsd;string"/>
            </owl:Restriction>
        </rdfs:subClassOf>
        <rdfs:subClassOf>
            <owl:Restriction>
                <owl:onProperty rdf:resource="&ns4;#partNumber"/>
                <owl:maxQualifiedCardinality rdf:datatype="&xsd;nonNegativeInteger">1</owl:maxQualifiedCardinality>
                <owl:onDataRange rdf:resource="&xsd;string"/>
            </owl:Restriction>
        </rdfs:subClassOf>
        <rdfs:subClassOf>
            <owl:Restriction>
                <owl:onProperty rdf:resource="&ns4;#script"/>
                <owl:maxQualifiedCardinality rdf:datatype="&xsd;nonNegativeInteger">1</owl:maxQualifiedCardinality>
                <owl:onDataRange rdf:resource="&xsd;string"/>
            </owl:Restriction>
        </rdfs:subClassOf>
        <rdfs:subClassOf>
            <owl:Restriction>
                <owl:onProperty rdf:resource="&ns4;#language"/>
                <owl:onClass rdf:resource="&ns4;#Language"/>
                <owl:maxQualifiedCardinality rdf:datatype="&xsd;nonNegativeInteger">1</owl:maxQualifiedCardinality>
            </owl:Restriction>
        </rdfs:subClassOf>
        <rdfs:subClassOf>
            <owl:Restriction>
                <owl:onProperty rdf:resource="&ns4;#title"/>
                <owl:allValuesFrom rdf:resource="&ns4;#Title"/>
            </owl:Restriction>
        </rdfs:subClassOf>
        <rdfs:subClassOf>
            <owl:Restriction>
                <owl:onProperty rdf:resource="&ns4;#displayLabel"/>
                <owl:maxQualifiedCardinality rdf:datatype="&xsd;nonNegativeInteger">1</owl:maxQualifiedCardinality>
                <owl:onDataRange rdf:resource="&xsd;string"/>
            </owl:Restriction>
        </rdfs:subClassOf>
        <rdfs:subClassOf>
            <owl:Restriction>
                <owl:onProperty rdf:resource="&ns4;#authorityURI"/>
                <owl:maxQualifiedCardinality rdf:datatype="&xsd;nonNegativeInteger">1</owl:maxQualifiedCardinality>
                <owl:onDataRange rdf:resource="&xsd;anyURI"/>
            </owl:Restriction>
        </rdfs:subClassOf>
        <rdfs:subClassOf>
            <owl:Restriction>
                <owl:onProperty rdf:resource="&ns4;#valueURI"/>
                <owl:maxQualifiedCardinality rdf:datatype="&xsd;nonNegativeInteger">1</owl:maxQualifiedCardinality>
                <owl:onDataRange rdf:resource="&xsd;anyURI"/>
            </owl:Restriction>
        </rdfs:subClassOf>
        <rdfs:comment>A term or phrase describing a collection, object, or object component. The title
      may be transcribed from the work, from previous metadata, or supplied.</rdfs:comment>
        <rdfs:comment>relatedTitle should be used to link to equivalent transliterated, translated,
      abbreviated, etc. titles.</rdfs:comment>
    </owl:Class>
    


    <!-- http://library.ucsd.edu/ontology/dams/#Vocabulary -->

    <owl:Class rdf:about="&ns4;#Vocabulary">
        <rdfs:label>Vocabulary</rdfs:label>
        <rdfs:subClassOf rdf:resource="&ns4;#DAMSThing"/>
        <rdfs:subClassOf>
            <owl:Restriction>
                <owl:onProperty rdf:resource="&ns4;#description"/>
                <owl:maxQualifiedCardinality rdf:datatype="&xsd;nonNegativeInteger">1</owl:maxQualifiedCardinality>
                <owl:onDataRange rdf:resource="&xsd;string"/>
            </owl:Restriction>
        </rdfs:subClassOf>
        <rdfs:comment>A collection of terms which can serve as values for a metadata element.</rdfs:comment>
    </owl:Class>
    


    <!-- http://library.ucsd.edu/ontology/dams/#VocabularyEntry -->

    <owl:Class rdf:about="&ns4;#VocabularyEntry">
        <rdfs:subClassOf rdf:resource="&ns4;#DAMSThing"/>
        <rdfs:subClassOf>
            <owl:Restriction>
                <owl:onProperty rdf:resource="&ns4;#vocabulary"/>
                <owl:onClass rdf:resource="&ns4;#Vocabulary"/>
                <owl:qualifiedCardinality rdf:datatype="&xsd;nonNegativeInteger">1</owl:qualifiedCardinality>
            </owl:Restriction>
        </rdfs:subClassOf>
        <rdfs:subClassOf>
            <owl:Restriction>
                <owl:onProperty rdf:resource="&ns4;#valueURI"/>
                <owl:maxQualifiedCardinality rdf:datatype="&xsd;nonNegativeInteger">1</owl:maxQualifiedCardinality>
                <owl:onDataRange rdf:resource="&xsd;anyURI"/>
            </owl:Restriction>
        </rdfs:subClassOf>
        <rdfs:subClassOf>
            <owl:Restriction>
                <owl:onProperty rdf:resource="&ns4;#authority"/>
                <owl:maxQualifiedCardinality rdf:datatype="&xsd;nonNegativeInteger">1</owl:maxQualifiedCardinality>
                <owl:onDataRange rdf:resource="&xsd;string"/>
            </owl:Restriction>
        </rdfs:subClassOf>
        <rdfs:subClassOf>
            <owl:Restriction>
                <owl:onProperty rdf:resource="&ns4;#authorityURI"/>
                <owl:maxQualifiedCardinality rdf:datatype="&xsd;nonNegativeInteger">1</owl:maxQualifiedCardinality>
                <owl:onDataRange rdf:resource="&xsd;anyURI"/>
            </owl:Restriction>
        </rdfs:subClassOf>
        <rdfs:subClassOf>
            <owl:Restriction>
                <owl:onProperty rdf:resource="&ns4;#description"/>
                <owl:maxQualifiedCardinality rdf:datatype="&xsd;nonNegativeInteger">1</owl:maxQualifiedCardinality>
                <owl:onDataRange rdf:resource="&xsd;string"/>
            </owl:Restriction>
        </rdfs:subClassOf>
        <rdfs:subClassOf>
            <owl:Restriction>
                <owl:onProperty rdf:resource="&ns4;#code"/>
                <owl:maxQualifiedCardinality rdf:datatype="&xsd;nonNegativeInteger">1</owl:maxQualifiedCardinality>
                <owl:onDataRange rdf:resource="&xsd;string"/>
            </owl:Restriction>
        </rdfs:subClassOf>
        <rdfs:subClassOf>
            <owl:Restriction>
                <owl:onProperty rdf:resource="&ns4;#value"/>
                <owl:qualifiedCardinality rdf:datatype="&xsd;nonNegativeInteger">1</owl:qualifiedCardinality>
                <owl:onDataRange rdf:resource="&xsd;string"/>
            </owl:Restriction>
        </rdfs:subClassOf>
        <rdfs:comment>Item in a controlled vocabulary list.</rdfs:comment>
    </owl:Class>
</rdf:RDF>



<!-- Generated by the OWL API (version 3.2.3.1824) http://owlapi.sourceforge.net -->

